failed to adjust the definition of alpha_equiv

qcp/ast/VC/alpha_equiv_goal.v
@@ -345,7 +345,7 @@ forall (t2_pre: Z) (t1_pre: Z) (term2: term) (term1: term) (z2: Z) (z1: Z) (y2: 
   &&  [| ((INT_MIN) <= 0) |]
 .
 
-Definition alpha_equiv_entail_wit_1 := 
+Definition alpha_equiv_entail_wit_1_1 := 
 forall (t2_pre: Z) (t1_pre: Z) (term2: term) (term1: term) ,
   [| ((termtypeID (term1)) = (termtypeID (term2))) |] 
   &&  [| (t1_pre <> 0) |] 
@@ -362,6 +362,54 @@ forall (t2_pre: Z) (t1_pre: Z) (term2: term) (term1: term) ,
   **  ((&((t2_pre)  # "term" ->ₛ "type")) # Int  |-> (termtypeID (term2)))
   **  (store_term' t1_pre term1 )
   **  (store_term' t2_pre term2 )
+|--
+  [| False |]
+  &&  emp
+.
+
+Definition alpha_equiv_entail_wit_1_2 := 
+forall (t2_pre: Z) (t1_pre: Z) (term2: term) (term1: term) (qt2: quant_type) (qv2: (@list Z)) (qterm2: term) (qt1: quant_type) (qv1: (@list Z)) (qterm1: term) (retval: Z) (str: (@list Z)) (z2: Z) (z1: Z) (y2: Z) (y1: Z) (qt2_2: quant_type) (qv2_2: (@list Z)) (qterm2_2: term) (qt1_2: quant_type) (qv1_2: (@list Z)) (qterm1_2: term) (retval_2: Z) (retval_3: Z) (retval_4: Z) (retval_5: Z) (retval_6: Z) ,
+  [| (retval_6 = (term_eqn ((term_subst_v (str) (qv1_2) (qterm1_2))) ((term_subst_v (str) (qv2_2) (qterm2_2))))) |] 
+  &&  [| (retval_5 = retval_4) |] 
+  &&  [| (retval_4 <> 0) |] 
+  &&  [| (retval_3 = retval_2) |] 
+  &&  [| (retval_2 <> 0) |] 
+  &&  [| (t1_pre <> 0) |] 
+  &&  [| (t2_pre <> 0) |] 
+  &&  [| (term1 = (TermQuant (qt1_2) (qv1_2) (qterm1_2))) |] 
+  &&  [| (term2 = (TermQuant (qt2_2) (qv2_2) (qterm2_2))) |] 
+  &&  [| (term_not_contain_var term1 str ) |] 
+  &&  [| (term_not_contain_var term2 str ) |] 
+  &&  [| (retval <> 0) |] 
+  &&  [| (retval = (list_Z_cmp (qv1) (qv2))) |] 
+  &&  [| ((qtID (qt1)) = (qtID (qt2))) |] 
+  &&  [| (t1_pre <> 0) |] 
+  &&  [| (t2_pre <> 0) |] 
+  &&  [| (term1 = (TermQuant (qt1) (qv1) (qterm1))) |] 
+  &&  [| (term2 = (TermQuant (qt2) (qv2) (qterm2))) |] 
+  &&  [| ((termtypeID (term1)) = (termtypeID (term2))) |] 
+  &&  [| (t1_pre <> 0) |] 
+  &&  [| (t2_pre <> 0) |] 
+  &&  [| (t2_pre <> 0) |] 
+  &&  [| (t1_pre <> 0) |] 
+  &&  [| ((termtypeID (term1)) <> 0) |] 
+  &&  [| ((termtypeID (term1)) <> 1) |] 
+  &&  [| ((termtypeID (term1)) <> 2) |] 
+  &&  [| ((termtypeID (term1)) = 3) |]
+  &&  (store_string y2 qv2_2 )
+  **  (store_term z2 qterm2_2 )
+  **  (store_string y1 qv1_2 )
+  **  (store_term z1 qterm1_2 )
+  **  ((( &( "t1" ) )) # Ptr  |-> t1_pre)
+  **  ((( &( "t2" ) )) # Ptr  |-> t2_pre)
+  **  ((&((t1_pre)  # "term" ->ₛ "type")) # Int  |-> (termtypeID (term1)))
+  **  ((&((t2_pre)  # "term" ->ₛ "type")) # Int  |-> (termtypeID (term2)))
+  **  ((&((t1_pre)  # "term" ->ₛ "content" .ₛ "Quant" .ₛ "type")) # Int  |-> (qtID (qt1_2)))
+  **  ((&((t2_pre)  # "term" ->ₛ "content" .ₛ "Quant" .ₛ "type")) # Int  |-> (qtID (qt2_2)))
+  **  ((&((t1_pre)  # "term" ->ₛ "content" .ₛ "Quant" .ₛ "var")) # Ptr  |-> y1)
+  **  ((&((t2_pre)  # "term" ->ₛ "content" .ₛ "Quant" .ₛ "var")) # Ptr  |-> y2)
+  **  ((&((t1_pre)  # "term" ->ₛ "content" .ₛ "Quant" .ₛ "body")) # Ptr  |-> z1)
+  **  ((&((t2_pre)  # "term" ->ₛ "content" .ₛ "Quant" .ₛ "body")) # Ptr  |-> z2)
 |--
   [| False |]
   &&  emp
@@ -699,48 +747,7 @@ forall (t2_pre: Z) (t1_pre: Z) (term2: term) (term1: term) (z2: Z) (z1: Z) (y2: 
   **  (store_term t2_pre term2 )
 .
 
-Definition alpha_equiv_return_wit_8 := 
-forall (t2_pre: Z) (t1_pre: Z) (term2: term) (term1: term) (z2: Z) (z1: Z) (y2: Z) (y1: Z) (qt2: quant_type) (qv2: (@list Z)) (qterm2: term) (qt1: quant_type) (qv1: (@list Z)) (qterm1: term) (retval_2: Z) (retval_3: Z) (retval_4: Z) (retval: Z) ,
-  [| (retval = (term_eqn (qterm1) ((term_subst_v (qv1) (qv2) (qterm2))))) |] 
-  &&  [| (retval_4 = retval_3) |] 
-  &&  [| (retval_3 <> 0) |] 
-  &&  [| (y1 <> 0) |] 
-  &&  [| (y2 <> 0) |] 
-  &&  [| (retval_2 <> 0) |] 
-  &&  [| (retval_2 = (list_Z_cmp (qv1) (qv2))) |] 
-  &&  [| ((qtID (qt1)) = (qtID (qt2))) |] 
-  &&  [| (t1_pre <> 0) |] 
-  &&  [| (t2_pre <> 0) |] 
-  &&  [| (term1 = (TermQuant (qt1) (qv1) (qterm1))) |] 
-  &&  [| (term2 = (TermQuant (qt2) (qv2) (qterm2))) |] 
-  &&  [| ((termtypeID (term1)) = (termtypeID (term2))) |] 
-  &&  [| (t1_pre <> 0) |] 
-  &&  [| (t2_pre <> 0) |] 
-  &&  [| (t2_pre <> 0) |] 
-  &&  [| (t1_pre <> 0) |] 
-  &&  [| ((termtypeID (term1)) <> 0) |] 
-  &&  [| ((termtypeID (term1)) <> 1) |] 
-  &&  [| ((termtypeID (term1)) <> 2) |] 
-  &&  [| ((termtypeID (term1)) = 3) |]
-  &&  (store_term z1 qterm1 )
-  **  (store_string y1 qv1 )
-  **  (store_string y2 qv2 )
-  **  (store_term z2 qterm2 )
-  **  ((&((t1_pre)  # "term" ->ₛ "content" .ₛ "Quant" .ₛ "var")) # Ptr  |-> y1)
-  **  ((&((t2_pre)  # "term" ->ₛ "content" .ₛ "Quant" .ₛ "var")) # Ptr  |-> y2)
-  **  ((&((t1_pre)  # "term" ->ₛ "type")) # Int  |-> (termtypeID (term1)))
-  **  ((&((t2_pre)  # "term" ->ₛ "type")) # Int  |-> (termtypeID (term2)))
-  **  ((&((t1_pre)  # "term" ->ₛ "content" .ₛ "Quant" .ₛ "type")) # Int  |-> (qtID (qt1)))
-  **  ((&((t2_pre)  # "term" ->ₛ "content" .ₛ "Quant" .ₛ "type")) # Int  |-> (qtID (qt2)))
-  **  ((&((t1_pre)  # "term" ->ₛ "content" .ₛ "Quant" .ₛ "body")) # Ptr  |-> z1)
-  **  ((&((t2_pre)  # "term" ->ₛ "content" .ₛ "Quant" .ₛ "body")) # Ptr  |-> z2)
-|--
-  [| (retval = (term_eqn (term1) (term2))) |]
-  &&  (store_term t1_pre term1 )
-  **  (store_term t2_pre term2 )
-.
-
-Definition alpha_equiv_return_wit_9_1 := 
+Definition alpha_equiv_return_wit_8_1 := 
 forall (t2_pre: Z) (t1_pre: Z) (term2: term) (term1: term) ,
   [| (t2_pre = 0) |] 
   &&  [| (t1_pre <> 0) |]
@@ -752,7 +759,7 @@ forall (t2_pre: Z) (t1_pre: Z) (term2: term) (term1: term) ,
   **  (store_term t2_pre term2 )
 .
 
-Definition alpha_equiv_return_wit_9_2 := 
+Definition alpha_equiv_return_wit_8_2 := 
 forall (t2_pre: Z) (t1_pre: Z) (term2: term) (term1: term) ,
   [| (t1_pre = 0) |]
   &&  (store_term t1_pre term1 )
@@ -763,7 +770,7 @@ forall (t2_pre: Z) (t1_pre: Z) (term2: term) (term1: term) ,
   **  (store_term t2_pre term2 )
 .
 
-Definition alpha_equiv_return_wit_10 := 
+Definition alpha_equiv_return_wit_9 := 
 forall (t2_pre: Z) (t1_pre: Z) (term2: term) (term1: term) ,
   [| ((termtypeID (term1)) <> (termtypeID (term2))) |] 
   &&  [| (t1_pre <> 0) |] 
@@ -1276,7 +1283,46 @@ forall (t2_pre: Z) (t1_pre: Z) (term2: term) (term1: term) (z2: Z) (z1: Z) (y2: 
   **  ((&((t2_pre)  # "term" ->ₛ "content" .ₛ "Quant" .ₛ "body")) # Ptr  |-> z2)
 .
 
-Definition alpha_equiv_partial_solve_wit_11 := 
+Definition alpha_equiv_partial_solve_wit_11_pure := 
+forall (t2_pre: Z) (t1_pre: Z) (term2: term) (term1: term) (z2: Z) (z1: Z) (y2: Z) (y1: Z) (qt2: quant_type) (qv2: (@list Z)) (qterm2: term) (qt1: quant_type) (qv1: (@list Z)) (qterm1: term) (retval: Z) ,
+  [| (retval <> 0) |] 
+  &&  [| (retval = (list_Z_cmp (qv1) (qv2))) |] 
+  &&  [| ((qtID (qt1)) = (qtID (qt2))) |] 
+  &&  [| (t1_pre <> 0) |] 
+  &&  [| (t2_pre <> 0) |] 
+  &&  [| (term1 = (TermQuant (qt1) (qv1) (qterm1))) |] 
+  &&  [| (term2 = (TermQuant (qt2) (qv2) (qterm2))) |] 
+  &&  [| ((termtypeID (term1)) = (termtypeID (term2))) |] 
+  &&  [| (t1_pre <> 0) |] 
+  &&  [| (t2_pre <> 0) |] 
+  &&  [| (t2_pre <> 0) |] 
+  &&  [| (t1_pre <> 0) |] 
+  &&  [| ((termtypeID (term1)) <> 0) |] 
+  &&  [| ((termtypeID (term1)) <> 1) |] 
+  &&  [| ((termtypeID (term1)) <> 2) |] 
+  &&  [| ((termtypeID (term1)) = 3) |]
+  &&  (store_string y1 qv1 )
+  **  (store_string y2 qv2 )
+  **  ((( &( "t1" ) )) # Ptr  |-> t1_pre)
+  **  ((( &( "t2" ) )) # Ptr  |-> t2_pre)
+  **  ((&((t1_pre)  # "term" ->ₛ "type")) # Int  |-> (termtypeID (term1)))
+  **  ((&((t2_pre)  # "term" ->ₛ "type")) # Int  |-> (termtypeID (term2)))
+  **  ((&((t1_pre)  # "term" ->ₛ "content" .ₛ "Quant" .ₛ "type")) # Int  |-> (qtID (qt1)))
+  **  ((&((t2_pre)  # "term" ->ₛ "content" .ₛ "Quant" .ₛ "type")) # Int  |-> (qtID (qt2)))
+  **  ((&((t1_pre)  # "term" ->ₛ "content" .ₛ "Quant" .ₛ "var")) # Ptr  |-> y1)
+  **  ((&((t2_pre)  # "term" ->ₛ "content" .ₛ "Quant" .ₛ "var")) # Ptr  |-> y2)
+  **  ((&((t1_pre)  # "term" ->ₛ "content" .ₛ "Quant" .ₛ "body")) # Ptr  |-> z1)
+  **  ((&((t2_pre)  # "term" ->ₛ "content" .ₛ "Quant" .ₛ "body")) # Ptr  |-> z2)
+  **  (store_term z1 qterm1 )
+  **  (store_term z2 qterm2 )
+|--
+  [| (t1_pre <> 0) |] 
+  &&  [| (t2_pre <> 0) |] 
+  &&  [| (term1 = (TermQuant (qt1) (qv1) (qterm1))) |] 
+  &&  [| (term2 = (TermQuant (qt2) (qv2) (qterm2))) |]
+.
+
+Definition alpha_equiv_partial_solve_wit_11_aux := 
 forall (t2_pre: Z) (t1_pre: Z) (term2: term) (term1: term) (z2: Z) (z1: Z) (y2: Z) (y1: Z) (qt2: quant_type) (qv2: (@list Z)) (qterm2: term) (qt1: quant_type) (qv1: (@list Z)) (qterm1: term) (retval: Z) ,
   [| (retval <> 0) |] 
   &&  [| (retval = (list_Z_cmp (qv1) (qv2))) |] 
@@ -1307,40 +1353,10 @@ forall (t2_pre: Z) (t1_pre: Z) (term2: term) (term1: term) (z2: Z) (z1: Z) (y2: 
   **  (store_term z1 qterm1 )
   **  (store_term z2 qterm2 )
 |--
-  [| (retval <> 0) |] 
-  &&  [| (retval = (list_Z_cmp (qv1) (qv2))) |] 
-  &&  [| ((qtID (qt1)) = (qtID (qt2))) |] 
-  &&  [| (t1_pre <> 0) |] 
+  [| (t1_pre <> 0) |] 
   &&  [| (t2_pre <> 0) |] 
   &&  [| (term1 = (TermQuant (qt1) (qv1) (qterm1))) |] 
   &&  [| (term2 = (TermQuant (qt2) (qv2) (qterm2))) |] 
-  &&  [| ((termtypeID (term1)) = (termtypeID (term2))) |] 
-  &&  [| (t1_pre <> 0) |] 
-  &&  [| (t2_pre <> 0) |] 
-  &&  [| (t2_pre <> 0) |] 
-  &&  [| (t1_pre <> 0) |] 
-  &&  [| ((termtypeID (term1)) <> 0) |] 
-  &&  [| ((termtypeID (term1)) <> 1) |] 
-  &&  [| ((termtypeID (term1)) <> 2) |] 
-  &&  [| ((termtypeID (term1)) = 3) |]
-  &&  ((&((t1_pre)  # "term" ->ₛ "content" .ₛ "Quant" .ₛ "var")) # Ptr  |-> y1)
-  **  (store_string y1 qv1 )
-  **  ((&((t2_pre)  # "term" ->ₛ "content" .ₛ "Quant" .ₛ "var")) # Ptr  |-> y2)
-  **  (store_string y2 qv2 )
-  **  ((&((t1_pre)  # "term" ->ₛ "type")) # Int  |-> (termtypeID (term1)))
-  **  ((&((t2_pre)  # "term" ->ₛ "type")) # Int  |-> (termtypeID (term2)))
-  **  ((&((t1_pre)  # "term" ->ₛ "content" .ₛ "Quant" .ₛ "type")) # Int  |-> (qtID (qt1)))
-  **  ((&((t2_pre)  # "term" ->ₛ "content" .ₛ "Quant" .ₛ "type")) # Int  |-> (qtID (qt2)))
-  **  ((&((t1_pre)  # "term" ->ₛ "content" .ₛ "Quant" .ₛ "body")) # Ptr  |-> z1)
-  **  ((&((t2_pre)  # "term" ->ₛ "content" .ₛ "Quant" .ₛ "body")) # Ptr  |-> z2)
-  **  (store_term z1 qterm1 )
-  **  (store_term z2 qterm2 )
-.
-
-Definition alpha_equiv_partial_solve_wit_12 := 
-forall (t2_pre: Z) (t1_pre: Z) (term2: term) (term1: term) (z2: Z) (z1: Z) (y2: Z) (y1: Z) (qt2: quant_type) (qv2: (@list Z)) (qterm2: term) (qt1: quant_type) (qv1: (@list Z)) (qterm1: term) (retval: Z) ,
-  [| (y1 <> 0) |] 
-  &&  [| (y2 <> 0) |] 
   &&  [| (retval <> 0) |] 
   &&  [| (retval = (list_Z_cmp (qv1) (qv2))) |] 
   &&  [| ((qtID (qt1)) = (qtID (qt2))) |] 
@@ -1357,56 +1373,818 @@ forall (t2_pre: Z) (t1_pre: Z) (term2: term) (term1: term) (z2: Z) (z1: Z) (y2: 
   &&  [| ((termtypeID (term1)) <> 1) |] 
   &&  [| ((termtypeID (term1)) <> 2) |] 
   &&  [| ((termtypeID (term1)) = 3) |]
-  &&  ((&((t1_pre)  # "term" ->ₛ "content" .ₛ "Quant" .ₛ "var")) # Ptr  |-> y1)
-  **  ((&((t2_pre)  # "term" ->ₛ "content" .ₛ "Quant" .ₛ "var")) # Ptr  |-> y2)
-  **  (store_string y1 qv1 )
-  **  (store_string y2 qv2 )
-  **  ((&((t1_pre)  # "term" ->ₛ "type")) # Int  |-> (termtypeID (term1)))
+  &&  ((&((t1_pre)  # "term" ->ₛ "type")) # Int  |-> (termtypeID (term1)))
   **  ((&((t2_pre)  # "term" ->ₛ "type")) # Int  |-> (termtypeID (term2)))
   **  ((&((t1_pre)  # "term" ->ₛ "content" .ₛ "Quant" .ₛ "type")) # Int  |-> (qtID (qt1)))
   **  ((&((t2_pre)  # "term" ->ₛ "content" .ₛ "Quant" .ₛ "type")) # Int  |-> (qtID (qt2)))
-  **  ((&((t1_pre)  # "term" ->ₛ "content" .ₛ "Quant" .ₛ "body")) # Ptr  |-> z1)
-  **  ((&((t2_pre)  # "term" ->ₛ "content" .ₛ "Quant" .ₛ "body")) # Ptr  |-> z2)
-  **  (store_term z1 qterm1 )
-  **  (store_term z2 qterm2 )
-|--
-  [| (y1 <> 0) |] 
-  &&  [| (y2 <> 0) |] 
-  &&  [| (retval <> 0) |] 
-  &&  [| (retval = (list_Z_cmp (qv1) (qv2))) |] 
-  &&  [| ((qtID (qt1)) = (qtID (qt2))) |] 
-  &&  [| (t1_pre <> 0) |] 
-  &&  [| (t2_pre <> 0) |] 
-  &&  [| (term1 = (TermQuant (qt1) (qv1) (qterm1))) |] 
-  &&  [| (term2 = (TermQuant (qt2) (qv2) (qterm2))) |] 
-  &&  [| ((termtypeID (term1)) = (termtypeID (term2))) |] 
-  &&  [| (t1_pre <> 0) |] 
-  &&  [| (t2_pre <> 0) |] 
-  &&  [| (t2_pre <> 0) |] 
-  &&  [| (t1_pre <> 0) |] 
-  &&  [| ((termtypeID (term1)) <> 0) |] 
-  &&  [| ((termtypeID (term1)) <> 1) |] 
-  &&  [| ((termtypeID (term1)) <> 2) |] 
-  &&  [| ((termtypeID (term1)) = 3) |]
-  &&  (store_term z2 qterm2 )
   **  ((&((t1_pre)  # "term" ->ₛ "content" .ₛ "Quant" .ₛ "var")) # Ptr  |-> y1)
   **  ((&((t2_pre)  # "term" ->ₛ "content" .ₛ "Quant" .ₛ "var")) # Ptr  |-> y2)
-  **  (store_string y1 qv1 )
-  **  (store_string y2 qv2 )
-  **  ((&((t1_pre)  # "term" ->ₛ "type")) # Int  |-> (termtypeID (term1)))
-  **  ((&((t2_pre)  # "term" ->ₛ "type")) # Int  |-> (termtypeID (term2)))
-  **  ((&((t1_pre)  # "term" ->ₛ "content" .ₛ "Quant" .ₛ "type")) # Int  |-> (qtID (qt1)))
-  **  ((&((t2_pre)  # "term" ->ₛ "content" .ₛ "Quant" .ₛ "type")) # Int  |-> (qtID (qt2)))
   **  ((&((t1_pre)  # "term" ->ₛ "content" .ₛ "Quant" .ₛ "body")) # Ptr  |-> z1)
   **  ((&((t2_pre)  # "term" ->ₛ "content" .ₛ "Quant" .ₛ "body")) # Ptr  |-> z2)
+  **  (store_string y1 qv1 )
   **  (store_term z1 qterm1 )
+  **  (store_string y2 qv2 )
+  **  (store_term z2 qterm2 )
 .
 
-Definition alpha_equiv_partial_solve_wit_13_pure := 
-forall (t2_pre: Z) (t1_pre: Z) (term2: term) (term1: term) (z2: Z) (z1: Z) (y2: Z) (y1: Z) (qt2: quant_type) (qv2: (@list Z)) (qterm2: term) (qt1: quant_type) (qv1: (@list Z)) (qterm1: term) (retval_2: Z) (retval: Z) ,
+Definition alpha_equiv_partial_solve_wit_11 := alpha_equiv_partial_solve_wit_11_pure -> alpha_equiv_partial_solve_wit_11_aux.
+
+Definition alpha_equiv_partial_solve_wit_12 := 
+forall (t2_pre: Z) (t1_pre: Z) (term2: term) (term1: term) (qt2: quant_type) (qv2: (@list Z)) (qterm2: term) (qt1: quant_type) (qv1: (@list Z)) (qterm1: term) (retval: Z) ,
   [| (retval <> 0) |] 
+  &&  [| (retval = (list_Z_cmp (qv1) (qv2))) |] 
+  &&  [| ((qtID (qt1)) = (qtID (qt2))) |] 
+  &&  [| (t1_pre <> 0) |] 
+  &&  [| (t2_pre <> 0) |] 
+  &&  [| (term1 = (TermQuant (qt1) (qv1) (qterm1))) |] 
+  &&  [| (term2 = (TermQuant (qt2) (qv2) (qterm2))) |] 
+  &&  [| ((termtypeID (term1)) = (termtypeID (term2))) |] 
+  &&  [| (t1_pre <> 0) |] 
+  &&  [| (t2_pre <> 0) |] 
+  &&  [| (t2_pre <> 0) |] 
+  &&  [| (t1_pre <> 0) |] 
+  &&  [| ((termtypeID (term1)) <> 0) |] 
+  &&  [| ((termtypeID (term1)) <> 1) |] 
+  &&  [| ((termtypeID (term1)) <> 2) |] 
+  &&  [| ((termtypeID (term1)) = 3) |]
+  &&  (store_term t1_pre term1 )
+  **  (store_term t2_pre term2 )
+|--
+  [| (retval <> 0) |] 
+  &&  [| (retval = (list_Z_cmp (qv1) (qv2))) |] 
+  &&  [| ((qtID (qt1)) = (qtID (qt2))) |] 
+  &&  [| (t1_pre <> 0) |] 
+  &&  [| (t2_pre <> 0) |] 
+  &&  [| (term1 = (TermQuant (qt1) (qv1) (qterm1))) |] 
+  &&  [| (term2 = (TermQuant (qt2) (qv2) (qterm2))) |] 
+  &&  [| ((termtypeID (term1)) = (termtypeID (term2))) |] 
+  &&  [| (t1_pre <> 0) |] 
+  &&  [| (t2_pre <> 0) |] 
+  &&  [| (t2_pre <> 0) |] 
+  &&  [| (t1_pre <> 0) |] 
+  &&  [| ((termtypeID (term1)) <> 0) |] 
+  &&  [| ((termtypeID (term1)) <> 1) |] 
+  &&  [| ((termtypeID (term1)) <> 2) |] 
+  &&  [| ((termtypeID (term1)) = 3) |]
+  &&  (store_term t1_pre term1 )
+  **  (store_term t2_pre term2 )
+.
+
+Definition alpha_equiv_partial_solve_wit_13 := 
+forall (t2_pre: Z) (t1_pre: Z) (term2: term) (term1: term) (qt2: quant_type) (qv2: (@list Z)) (qterm2: term) (qt1: quant_type) (qv1: (@list Z)) (qterm1: term) (retval: Z) (str: (@list Z)) (retval_2: Z) ,
+  [| (term_not_contain_var term1 str ) |] 
+  &&  [| (term_not_contain_var term2 str ) |] 
+  &&  [| (retval <> 0) |] 
+  &&  [| (retval = (list_Z_cmp (qv1) (qv2))) |] 
+  &&  [| ((qtID (qt1)) = (qtID (qt2))) |] 
+  &&  [| (t1_pre <> 0) |] 
+  &&  [| (t2_pre <> 0) |] 
+  &&  [| (term1 = (TermQuant (qt1) (qv1) (qterm1))) |] 
+  &&  [| (term2 = (TermQuant (qt2) (qv2) (qterm2))) |] 
+  &&  [| ((termtypeID (term1)) = (termtypeID (term2))) |] 
+  &&  [| (t1_pre <> 0) |] 
+  &&  [| (t2_pre <> 0) |] 
+  &&  [| (t2_pre <> 0) |] 
+  &&  [| (t1_pre <> 0) |] 
+  &&  [| ((termtypeID (term1)) <> 0) |] 
+  &&  [| ((termtypeID (term1)) <> 1) |] 
+  &&  [| ((termtypeID (term1)) <> 2) |] 
+  &&  [| ((termtypeID (term1)) = 3) |]
+  &&  (store_term t1_pre term1 )
+  **  (store_term t2_pre term2 )
+  **  (store_string retval_2 str )
+|--
+  [| (term_not_contain_var term1 str ) |] 
+  &&  [| (term_not_contain_var term2 str ) |] 
+  &&  [| (retval <> 0) |] 
+  &&  [| (retval = (list_Z_cmp (qv1) (qv2))) |] 
+  &&  [| ((qtID (qt1)) = (qtID (qt2))) |] 
+  &&  [| (t1_pre <> 0) |] 
+  &&  [| (t2_pre <> 0) |] 
+  &&  [| (term1 = (TermQuant (qt1) (qv1) (qterm1))) |] 
+  &&  [| (term2 = (TermQuant (qt2) (qv2) (qterm2))) |] 
+  &&  [| ((termtypeID (term1)) = (termtypeID (term2))) |] 
+  &&  [| (t1_pre <> 0) |] 
+  &&  [| (t2_pre <> 0) |] 
+  &&  [| (t2_pre <> 0) |] 
+  &&  [| (t1_pre <> 0) |] 
+  &&  [| ((termtypeID (term1)) <> 0) |] 
+  &&  [| ((termtypeID (term1)) <> 1) |] 
+  &&  [| ((termtypeID (term1)) <> 2) |] 
+  &&  [| ((termtypeID (term1)) = 3) |]
+  &&  (store_term t1_pre term1 )
+  **  (store_term t2_pre term2 )
+  **  (store_string retval_2 str )
+.
+
+Definition alpha_equiv_partial_solve_wit_14 := 
+forall (t2_pre: Z) (t1_pre: Z) (term2: term) (term1: term) (qt2: quant_type) (qv2: (@list Z)) (qterm2: term) (qt1: quant_type) (qv1: (@list Z)) (qterm1: term) (retval: Z) (str: (@list Z)) (retval_2: Z) (z2: Z) (z1: Z) (y2: Z) (y1: Z) (qt2_2: quant_type) (qv2_2: (@list Z)) (qterm2_2: term) (qt1_2: quant_type) (qv1_2: (@list Z)) (qterm1_2: term) ,
+  [| (t1_pre <> 0) |] 
+  &&  [| (t2_pre <> 0) |] 
+  &&  [| (term1 = (TermQuant (qt1_2) (qv1_2) (qterm1_2))) |] 
+  &&  [| (term2 = (TermQuant (qt2_2) (qv2_2) (qterm2_2))) |] 
+  &&  [| (term_not_contain_var term1 str ) |] 
+  &&  [| (term_not_contain_var term2 str ) |] 
+  &&  [| (retval <> 0) |] 
+  &&  [| (retval = (list_Z_cmp (qv1) (qv2))) |] 
+  &&  [| ((qtID (qt1)) = (qtID (qt2))) |] 
+  &&  [| (t1_pre <> 0) |] 
+  &&  [| (t2_pre <> 0) |] 
+  &&  [| (term1 = (TermQuant (qt1) (qv1) (qterm1))) |] 
+  &&  [| (term2 = (TermQuant (qt2) (qv2) (qterm2))) |] 
+  &&  [| ((termtypeID (term1)) = (termtypeID (term2))) |] 
+  &&  [| (t1_pre <> 0) |] 
+  &&  [| (t2_pre <> 0) |] 
+  &&  [| (t2_pre <> 0) |] 
+  &&  [| (t1_pre <> 0) |] 
+  &&  [| ((termtypeID (term1)) <> 0) |] 
+  &&  [| ((termtypeID (term1)) <> 1) |] 
+  &&  [| ((termtypeID (term1)) <> 2) |] 
+  &&  [| ((termtypeID (term1)) = 3) |]
+  &&  ((&((t1_pre)  # "term" ->ₛ "type")) # Int  |-> (termtypeID (term1)))
+  **  ((&((t2_pre)  # "term" ->ₛ "type")) # Int  |-> (termtypeID (term2)))
+  **  ((&((t1_pre)  # "term" ->ₛ "content" .ₛ "Quant" .ₛ "type")) # Int  |-> (qtID (qt1_2)))
+  **  ((&((t2_pre)  # "term" ->ₛ "content" .ₛ "Quant" .ₛ "type")) # Int  |-> (qtID (qt2_2)))
+  **  ((&((t1_pre)  # "term" ->ₛ "content" .ₛ "Quant" .ₛ "var")) # Ptr  |-> y1)
+  **  ((&((t2_pre)  # "term" ->ₛ "content" .ₛ "Quant" .ₛ "var")) # Ptr  |-> y2)
+  **  ((&((t1_pre)  # "term" ->ₛ "content" .ₛ "Quant" .ₛ "body")) # Ptr  |-> z1)
+  **  ((&((t2_pre)  # "term" ->ₛ "content" .ₛ "Quant" .ₛ "body")) # Ptr  |-> z2)
+  **  (store_string y1 qv1_2 )
+  **  (store_term z1 qterm1_2 )
+  **  (store_string y2 qv2_2 )
+  **  (store_term z2 qterm2_2 )
+  **  (store_string retval_2 str )
+|--
+  [| (t1_pre <> 0) |] 
+  &&  [| (t2_pre <> 0) |] 
+  &&  [| (term1 = (TermQuant (qt1_2) (qv1_2) (qterm1_2))) |] 
+  &&  [| (term2 = (TermQuant (qt2_2) (qv2_2) (qterm2_2))) |] 
+  &&  [| (term_not_contain_var term1 str ) |] 
+  &&  [| (term_not_contain_var term2 str ) |] 
+  &&  [| (retval <> 0) |] 
+  &&  [| (retval = (list_Z_cmp (qv1) (qv2))) |] 
+  &&  [| ((qtID (qt1)) = (qtID (qt2))) |] 
+  &&  [| (t1_pre <> 0) |] 
+  &&  [| (t2_pre <> 0) |] 
+  &&  [| (term1 = (TermQuant (qt1) (qv1) (qterm1))) |] 
+  &&  [| (term2 = (TermQuant (qt2) (qv2) (qterm2))) |] 
+  &&  [| ((termtypeID (term1)) = (termtypeID (term2))) |] 
+  &&  [| (t1_pre <> 0) |] 
+  &&  [| (t2_pre <> 0) |] 
+  &&  [| (t2_pre <> 0) |] 
+  &&  [| (t1_pre <> 0) |] 
+  &&  [| ((termtypeID (term1)) <> 0) |] 
+  &&  [| ((termtypeID (term1)) <> 1) |] 
+  &&  [| ((termtypeID (term1)) <> 2) |] 
+  &&  [| ((termtypeID (term1)) = 3) |]
+  &&  (store_term z1 qterm1_2 )
+  **  ((&((t1_pre)  # "term" ->ₛ "type")) # Int  |-> (termtypeID (term1)))
+  **  ((&((t2_pre)  # "term" ->ₛ "type")) # Int  |-> (termtypeID (term2)))
+  **  ((&((t1_pre)  # "term" ->ₛ "content" .ₛ "Quant" .ₛ "type")) # Int  |-> (qtID (qt1_2)))
+  **  ((&((t2_pre)  # "term" ->ₛ "content" .ₛ "Quant" .ₛ "type")) # Int  |-> (qtID (qt2_2)))
+  **  ((&((t1_pre)  # "term" ->ₛ "content" .ₛ "Quant" .ₛ "var")) # Ptr  |-> y1)
+  **  ((&((t2_pre)  # "term" ->ₛ "content" .ₛ "Quant" .ₛ "var")) # Ptr  |-> y2)
+  **  ((&((t1_pre)  # "term" ->ₛ "content" .ₛ "Quant" .ₛ "body")) # Ptr  |-> z1)
+  **  ((&((t2_pre)  # "term" ->ₛ "content" .ₛ "Quant" .ₛ "body")) # Ptr  |-> z2)
+  **  (store_string y1 qv1_2 )
+  **  (store_string y2 qv2_2 )
+  **  (store_term z2 qterm2_2 )
+  **  (store_string retval_2 str )
+.
+
+Definition alpha_equiv_partial_solve_wit_15_pure := 
+forall (t2_pre: Z) (t1_pre: Z) (term2: term) (term1: term) (qt2: quant_type) (qv2: (@list Z)) (qterm2: term) (qt1: quant_type) (qv1: (@list Z)) (qterm1: term) (retval_3: Z) (str: (@list Z)) (retval: Z) (z2: Z) (z1: Z) (y2: Z) (y1: Z) (qt2_2: quant_type) (qv2_2: (@list Z)) (qterm2_2: term) (qt1_2: quant_type) (qv1_2: (@list Z)) (qterm1_2: term) (retval_2: Z) ,
+  [| (retval_2 <> 0) |] 
+  &&  [| (t1_pre <> 0) |] 
+  &&  [| (t2_pre <> 0) |] 
+  &&  [| (term1 = (TermQuant (qt1_2) (qv1_2) (qterm1_2))) |] 
+  &&  [| (term2 = (TermQuant (qt2_2) (qv2_2) (qterm2_2))) |] 
+  &&  [| (term_not_contain_var term1 str ) |] 
+  &&  [| (term_not_contain_var term2 str ) |] 
+  &&  [| (retval_3 <> 0) |] 
+  &&  [| (retval_3 = (list_Z_cmp (qv1) (qv2))) |] 
+  &&  [| ((qtID (qt1)) = (qtID (qt2))) |] 
+  &&  [| (t1_pre <> 0) |] 
+  &&  [| (t2_pre <> 0) |] 
+  &&  [| (term1 = (TermQuant (qt1) (qv1) (qterm1))) |] 
+  &&  [| (term2 = (TermQuant (qt2) (qv2) (qterm2))) |] 
+  &&  [| ((termtypeID (term1)) = (termtypeID (term2))) |] 
+  &&  [| (t1_pre <> 0) |] 
+  &&  [| (t2_pre <> 0) |] 
+  &&  [| (t2_pre <> 0) |] 
+  &&  [| (t1_pre <> 0) |] 
+  &&  [| ((termtypeID (term1)) <> 0) |] 
+  &&  [| ((termtypeID (term1)) <> 1) |] 
+  &&  [| ((termtypeID (term1)) <> 2) |] 
+  &&  [| ((termtypeID (term1)) = 3) |]
+  &&  (store_term z1 qterm1_2 )
+  **  (store_term retval_2 qterm1_2 )
+  **  ((( &( "new_t1" ) )) # Ptr  |->_)
+  **  ((( &( "t1" ) )) # Ptr  |-> t1_pre)
+  **  ((( &( "t2" ) )) # Ptr  |-> t2_pre)
+  **  ((&((t1_pre)  # "term" ->ₛ "type")) # Int  |-> (termtypeID (term1)))
+  **  ((&((t2_pre)  # "term" ->ₛ "type")) # Int  |-> (termtypeID (term2)))
+  **  ((&((t1_pre)  # "term" ->ₛ "content" .ₛ "Quant" .ₛ "type")) # Int  |-> (qtID (qt1_2)))
+  **  ((&((t2_pre)  # "term" ->ₛ "content" .ₛ "Quant" .ₛ "type")) # Int  |-> (qtID (qt2_2)))
+  **  ((&((t1_pre)  # "term" ->ₛ "content" .ₛ "Quant" .ₛ "var")) # Ptr  |-> y1)
+  **  ((&((t2_pre)  # "term" ->ₛ "content" .ₛ "Quant" .ₛ "var")) # Ptr  |-> y2)
+  **  ((&((t1_pre)  # "term" ->ₛ "content" .ₛ "Quant" .ₛ "body")) # Ptr  |-> z1)
+  **  ((&((t2_pre)  # "term" ->ₛ "content" .ₛ "Quant" .ₛ "body")) # Ptr  |-> z2)
+  **  (store_string y1 qv1_2 )
+  **  (store_string y2 qv2_2 )
+  **  (store_term z2 qterm2_2 )
+  **  (store_string retval str )
+  **  ((( &( "new_var" ) )) # Ptr  |-> retval)
+|--
+  [| (retval_2 <> 0) |] 
   &&  [| (y1 <> 0) |] 
+  &&  [| (retval <> 0) |]
+.
+
+Definition alpha_equiv_partial_solve_wit_15_aux := 
+forall (t2_pre: Z) (t1_pre: Z) (term2: term) (term1: term) (qt2: quant_type) (qv2: (@list Z)) (qterm2: term) (qt1: quant_type) (qv1: (@list Z)) (qterm1: term) (retval: Z) (str: (@list Z)) (retval_2: Z) (z2: Z) (z1: Z) (y2: Z) (y1: Z) (qt2_2: quant_type) (qv2_2: (@list Z)) (qterm2_2: term) (qt1_2: quant_type) (qv1_2: (@list Z)) (qterm1_2: term) (retval_3: Z) ,
+  [| (retval_3 <> 0) |] 
+  &&  [| (t1_pre <> 0) |] 
+  &&  [| (t2_pre <> 0) |] 
+  &&  [| (term1 = (TermQuant (qt1_2) (qv1_2) (qterm1_2))) |] 
+  &&  [| (term2 = (TermQuant (qt2_2) (qv2_2) (qterm2_2))) |] 
+  &&  [| (term_not_contain_var term1 str ) |] 
+  &&  [| (term_not_contain_var term2 str ) |] 
+  &&  [| (retval <> 0) |] 
+  &&  [| (retval = (list_Z_cmp (qv1) (qv2))) |] 
+  &&  [| ((qtID (qt1)) = (qtID (qt2))) |] 
+  &&  [| (t1_pre <> 0) |] 
+  &&  [| (t2_pre <> 0) |] 
+  &&  [| (term1 = (TermQuant (qt1) (qv1) (qterm1))) |] 
+  &&  [| (term2 = (TermQuant (qt2) (qv2) (qterm2))) |] 
+  &&  [| ((termtypeID (term1)) = (termtypeID (term2))) |] 
+  &&  [| (t1_pre <> 0) |] 
+  &&  [| (t2_pre <> 0) |] 
+  &&  [| (t2_pre <> 0) |] 
+  &&  [| (t1_pre <> 0) |] 
+  &&  [| ((termtypeID (term1)) <> 0) |] 
+  &&  [| ((termtypeID (term1)) <> 1) |] 
+  &&  [| ((termtypeID (term1)) <> 2) |] 
+  &&  [| ((termtypeID (term1)) = 3) |]
+  &&  (store_term z1 qterm1_2 )
+  **  (store_term retval_3 qterm1_2 )
+  **  ((&((t1_pre)  # "term" ->ₛ "type")) # Int  |-> (termtypeID (term1)))
+  **  ((&((t2_pre)  # "term" ->ₛ "type")) # Int  |-> (termtypeID (term2)))
+  **  ((&((t1_pre)  # "term" ->ₛ "content" .ₛ "Quant" .ₛ "type")) # Int  |-> (qtID (qt1_2)))
+  **  ((&((t2_pre)  # "term" ->ₛ "content" .ₛ "Quant" .ₛ "type")) # Int  |-> (qtID (qt2_2)))
+  **  ((&((t1_pre)  # "term" ->ₛ "content" .ₛ "Quant" .ₛ "var")) # Ptr  |-> y1)
+  **  ((&((t2_pre)  # "term" ->ₛ "content" .ₛ "Quant" .ₛ "var")) # Ptr  |-> y2)
+  **  ((&((t1_pre)  # "term" ->ₛ "content" .ₛ "Quant" .ₛ "body")) # Ptr  |-> z1)
+  **  ((&((t2_pre)  # "term" ->ₛ "content" .ₛ "Quant" .ₛ "body")) # Ptr  |-> z2)
+  **  (store_string y1 qv1_2 )
+  **  (store_string y2 qv2_2 )
+  **  (store_term z2 qterm2_2 )
+  **  (store_string retval_2 str )
+|--
+  [| (retval_3 <> 0) |] 
+  &&  [| (y1 <> 0) |] 
+  &&  [| (retval_2 <> 0) |] 
+  &&  [| (retval_3 <> 0) |] 
+  &&  [| (t1_pre <> 0) |] 
+  &&  [| (t2_pre <> 0) |] 
+  &&  [| (term1 = (TermQuant (qt1_2) (qv1_2) (qterm1_2))) |] 
+  &&  [| (term2 = (TermQuant (qt2_2) (qv2_2) (qterm2_2))) |] 
+  &&  [| (term_not_contain_var term1 str ) |] 
+  &&  [| (term_not_contain_var term2 str ) |] 
+  &&  [| (retval <> 0) |] 
+  &&  [| (retval = (list_Z_cmp (qv1) (qv2))) |] 
+  &&  [| ((qtID (qt1)) = (qtID (qt2))) |] 
+  &&  [| (t1_pre <> 0) |] 
+  &&  [| (t2_pre <> 0) |] 
+  &&  [| (term1 = (TermQuant (qt1) (qv1) (qterm1))) |] 
+  &&  [| (term2 = (TermQuant (qt2) (qv2) (qterm2))) |] 
+  &&  [| ((termtypeID (term1)) = (termtypeID (term2))) |] 
+  &&  [| (t1_pre <> 0) |] 
+  &&  [| (t2_pre <> 0) |] 
+  &&  [| (t2_pre <> 0) |] 
+  &&  [| (t1_pre <> 0) |] 
+  &&  [| ((termtypeID (term1)) <> 0) |] 
+  &&  [| ((termtypeID (term1)) <> 1) |] 
+  &&  [| ((termtypeID (term1)) <> 2) |] 
+  &&  [| ((termtypeID (term1)) = 3) |]
+  &&  (store_term retval_3 qterm1_2 )
+  **  (store_string y1 qv1_2 )
+  **  (store_string retval_2 str )
+  **  (store_term z1 qterm1_2 )
+  **  ((&((t1_pre)  # "term" ->ₛ "type")) # Int  |-> (termtypeID (term1)))
+  **  ((&((t2_pre)  # "term" ->ₛ "type")) # Int  |-> (termtypeID (term2)))
+  **  ((&((t1_pre)  # "term" ->ₛ "content" .ₛ "Quant" .ₛ "type")) # Int  |-> (qtID (qt1_2)))
+  **  ((&((t2_pre)  # "term" ->ₛ "content" .ₛ "Quant" .ₛ "type")) # Int  |-> (qtID (qt2_2)))
+  **  ((&((t1_pre)  # "term" ->ₛ "content" .ₛ "Quant" .ₛ "var")) # Ptr  |-> y1)
+  **  ((&((t2_pre)  # "term" ->ₛ "content" .ₛ "Quant" .ₛ "var")) # Ptr  |-> y2)
+  **  ((&((t1_pre)  # "term" ->ₛ "content" .ₛ "Quant" .ₛ "body")) # Ptr  |-> z1)
+  **  ((&((t2_pre)  # "term" ->ₛ "content" .ₛ "Quant" .ₛ "body")) # Ptr  |-> z2)
+  **  (store_string y2 qv2_2 )
+  **  (store_term z2 qterm2_2 )
+.
+
+Definition alpha_equiv_partial_solve_wit_15 := alpha_equiv_partial_solve_wit_15_pure -> alpha_equiv_partial_solve_wit_15_aux.
+
+Definition alpha_equiv_partial_solve_wit_16 := 
+forall (t2_pre: Z) (t1_pre: Z) (term2: term) (term1: term) (qt2: quant_type) (qv2: (@list Z)) (qterm2: term) (qt1: quant_type) (qv1: (@list Z)) (qterm1: term) (retval: Z) (str: (@list Z)) (retval_2: Z) (z2: Z) (z1: Z) (y2: Z) (y1: Z) (qt2_2: quant_type) (qv2_2: (@list Z)) (qterm2_2: term) (qt1_2: quant_type) (qv1_2: (@list Z)) (qterm1_2: term) (retval_3: Z) (retval_4: Z) ,
+  [| (retval_4 = retval_3) |] 
+  &&  [| (retval_3 <> 0) |] 
+  &&  [| (t1_pre <> 0) |] 
+  &&  [| (t2_pre <> 0) |] 
+  &&  [| (term1 = (TermQuant (qt1_2) (qv1_2) (qterm1_2))) |] 
+  &&  [| (term2 = (TermQuant (qt2_2) (qv2_2) (qterm2_2))) |] 
+  &&  [| (term_not_contain_var term1 str ) |] 
+  &&  [| (term_not_contain_var term2 str ) |] 
+  &&  [| (retval <> 0) |] 
+  &&  [| (retval = (list_Z_cmp (qv1) (qv2))) |] 
+  &&  [| ((qtID (qt1)) = (qtID (qt2))) |] 
+  &&  [| (t1_pre <> 0) |] 
+  &&  [| (t2_pre <> 0) |] 
+  &&  [| (term1 = (TermQuant (qt1) (qv1) (qterm1))) |] 
+  &&  [| (term2 = (TermQuant (qt2) (qv2) (qterm2))) |] 
+  &&  [| ((termtypeID (term1)) = (termtypeID (term2))) |] 
+  &&  [| (t1_pre <> 0) |] 
+  &&  [| (t2_pre <> 0) |] 
+  &&  [| (t2_pre <> 0) |] 
+  &&  [| (t1_pre <> 0) |] 
+  &&  [| ((termtypeID (term1)) <> 0) |] 
+  &&  [| ((termtypeID (term1)) <> 1) |] 
+  &&  [| ((termtypeID (term1)) <> 2) |] 
+  &&  [| ((termtypeID (term1)) = 3) |]
+  &&  (store_term retval_3 (term_subst_v (str) (qv1_2) (qterm1_2)) )
+  **  (store_string retval_2 str )
+  **  (store_string y1 qv1_2 )
+  **  (store_term z1 qterm1_2 )
+  **  ((&((t1_pre)  # "term" ->ₛ "type")) # Int  |-> (termtypeID (term1)))
+  **  ((&((t2_pre)  # "term" ->ₛ "type")) # Int  |-> (termtypeID (term2)))
+  **  ((&((t1_pre)  # "term" ->ₛ "content" .ₛ "Quant" .ₛ "type")) # Int  |-> (qtID (qt1_2)))
+  **  ((&((t2_pre)  # "term" ->ₛ "content" .ₛ "Quant" .ₛ "type")) # Int  |-> (qtID (qt2_2)))
+  **  ((&((t1_pre)  # "term" ->ₛ "content" .ₛ "Quant" .ₛ "var")) # Ptr  |-> y1)
+  **  ((&((t2_pre)  # "term" ->ₛ "content" .ₛ "Quant" .ₛ "var")) # Ptr  |-> y2)
+  **  ((&((t1_pre)  # "term" ->ₛ "content" .ₛ "Quant" .ₛ "body")) # Ptr  |-> z1)
+  **  ((&((t2_pre)  # "term" ->ₛ "content" .ₛ "Quant" .ₛ "body")) # Ptr  |-> z2)
+  **  (store_string y2 qv2_2 )
+  **  (store_term z2 qterm2_2 )
+|--
+  [| (retval_4 = retval_3) |] 
+  &&  [| (retval_3 <> 0) |] 
+  &&  [| (t1_pre <> 0) |] 
+  &&  [| (t2_pre <> 0) |] 
+  &&  [| (term1 = (TermQuant (qt1_2) (qv1_2) (qterm1_2))) |] 
+  &&  [| (term2 = (TermQuant (qt2_2) (qv2_2) (qterm2_2))) |] 
+  &&  [| (term_not_contain_var term1 str ) |] 
+  &&  [| (term_not_contain_var term2 str ) |] 
+  &&  [| (retval <> 0) |] 
+  &&  [| (retval = (list_Z_cmp (qv1) (qv2))) |] 
+  &&  [| ((qtID (qt1)) = (qtID (qt2))) |] 
+  &&  [| (t1_pre <> 0) |] 
+  &&  [| (t2_pre <> 0) |] 
+  &&  [| (term1 = (TermQuant (qt1) (qv1) (qterm1))) |] 
+  &&  [| (term2 = (TermQuant (qt2) (qv2) (qterm2))) |] 
+  &&  [| ((termtypeID (term1)) = (termtypeID (term2))) |] 
+  &&  [| (t1_pre <> 0) |] 
+  &&  [| (t2_pre <> 0) |] 
+  &&  [| (t2_pre <> 0) |] 
+  &&  [| (t1_pre <> 0) |] 
+  &&  [| ((termtypeID (term1)) <> 0) |] 
+  &&  [| ((termtypeID (term1)) <> 1) |] 
+  &&  [| ((termtypeID (term1)) <> 2) |] 
+  &&  [| ((termtypeID (term1)) = 3) |]
+  &&  (store_term z2 qterm2_2 )
+  **  (store_term retval_3 (term_subst_v (str) (qv1_2) (qterm1_2)) )
+  **  (store_string retval_2 str )
+  **  (store_string y1 qv1_2 )
+  **  (store_term z1 qterm1_2 )
+  **  ((&((t1_pre)  # "term" ->ₛ "type")) # Int  |-> (termtypeID (term1)))
+  **  ((&((t2_pre)  # "term" ->ₛ "type")) # Int  |-> (termtypeID (term2)))
+  **  ((&((t1_pre)  # "term" ->ₛ "content" .ₛ "Quant" .ₛ "type")) # Int  |-> (qtID (qt1_2)))
+  **  ((&((t2_pre)  # "term" ->ₛ "content" .ₛ "Quant" .ₛ "type")) # Int  |-> (qtID (qt2_2)))
+  **  ((&((t1_pre)  # "term" ->ₛ "content" .ₛ "Quant" .ₛ "var")) # Ptr  |-> y1)
+  **  ((&((t2_pre)  # "term" ->ₛ "content" .ₛ "Quant" .ₛ "var")) # Ptr  |-> y2)
+  **  ((&((t1_pre)  # "term" ->ₛ "content" .ₛ "Quant" .ₛ "body")) # Ptr  |-> z1)
+  **  ((&((t2_pre)  # "term" ->ₛ "content" .ₛ "Quant" .ₛ "body")) # Ptr  |-> z2)
+  **  (store_string y2 qv2_2 )
+.
+
+Definition alpha_equiv_partial_solve_wit_17_pure := 
+forall (t2_pre: Z) (t1_pre: Z) (term2: term) (term1: term) (qt2: quant_type) (qv2: (@list Z)) (qterm2: term) (qt1: quant_type) (qv1: (@list Z)) (qterm1: term) (retval_3: Z) (str: (@list Z)) (retval: Z) (z2: Z) (z1: Z) (y2: Z) (y1: Z) (qt2_2: quant_type) (qv2_2: (@list Z)) (qterm2_2: term) (qt1_2: quant_type) (qv1_2: (@list Z)) (qterm1_2: term) (retval_4: Z) (retval_5: Z) (retval_2: Z) ,
+  [| (retval_2 <> 0) |] 
+  &&  [| (retval_5 = retval_4) |] 
+  &&  [| (retval_4 <> 0) |] 
+  &&  [| (t1_pre <> 0) |] 
+  &&  [| (t2_pre <> 0) |] 
+  &&  [| (term1 = (TermQuant (qt1_2) (qv1_2) (qterm1_2))) |] 
+  &&  [| (term2 = (TermQuant (qt2_2) (qv2_2) (qterm2_2))) |] 
+  &&  [| (term_not_contain_var term1 str ) |] 
+  &&  [| (term_not_contain_var term2 str ) |] 
+  &&  [| (retval_3 <> 0) |] 
+  &&  [| (retval_3 = (list_Z_cmp (qv1) (qv2))) |] 
+  &&  [| ((qtID (qt1)) = (qtID (qt2))) |] 
+  &&  [| (t1_pre <> 0) |] 
+  &&  [| (t2_pre <> 0) |] 
+  &&  [| (term1 = (TermQuant (qt1) (qv1) (qterm1))) |] 
+  &&  [| (term2 = (TermQuant (qt2) (qv2) (qterm2))) |] 
+  &&  [| ((termtypeID (term1)) = (termtypeID (term2))) |] 
+  &&  [| (t1_pre <> 0) |] 
+  &&  [| (t2_pre <> 0) |] 
+  &&  [| (t2_pre <> 0) |] 
+  &&  [| (t1_pre <> 0) |] 
+  &&  [| ((termtypeID (term1)) <> 0) |] 
+  &&  [| ((termtypeID (term1)) <> 1) |] 
+  &&  [| ((termtypeID (term1)) <> 2) |] 
+  &&  [| ((termtypeID (term1)) = 3) |]
+  &&  (store_term z2 qterm2_2 )
+  **  (store_term retval_2 qterm2_2 )
+  **  ((( &( "new_t2" ) )) # Ptr  |->_)
+  **  (store_term retval_4 (term_subst_v (str) (qv1_2) (qterm1_2)) )
+  **  (store_string retval str )
+  **  (store_string y1 qv1_2 )
+  **  (store_term z1 qterm1_2 )
+  **  ((( &( "new_t1" ) )) # Ptr  |-> retval_5)
+  **  ((( &( "t1" ) )) # Ptr  |-> t1_pre)
+  **  ((( &( "t2" ) )) # Ptr  |-> t2_pre)
+  **  ((&((t1_pre)  # "term" ->ₛ "type")) # Int  |-> (termtypeID (term1)))
+  **  ((&((t2_pre)  # "term" ->ₛ "type")) # Int  |-> (termtypeID (term2)))
+  **  ((&((t1_pre)  # "term" ->ₛ "content" .ₛ "Quant" .ₛ "type")) # Int  |-> (qtID (qt1_2)))
+  **  ((&((t2_pre)  # "term" ->ₛ "content" .ₛ "Quant" .ₛ "type")) # Int  |-> (qtID (qt2_2)))
+  **  ((&((t1_pre)  # "term" ->ₛ "content" .ₛ "Quant" .ₛ "var")) # Ptr  |-> y1)
+  **  ((&((t2_pre)  # "term" ->ₛ "content" .ₛ "Quant" .ₛ "var")) # Ptr  |-> y2)
+  **  ((&((t1_pre)  # "term" ->ₛ "content" .ₛ "Quant" .ₛ "body")) # Ptr  |-> z1)
+  **  ((&((t2_pre)  # "term" ->ₛ "content" .ₛ "Quant" .ₛ "body")) # Ptr  |-> z2)
+  **  (store_string y2 qv2_2 )
+  **  ((( &( "new_var" ) )) # Ptr  |-> retval)
+|--
+  [| (retval_2 <> 0) |] 
   &&  [| (y2 <> 0) |] 
+  &&  [| (retval <> 0) |]
+.
+
+Definition alpha_equiv_partial_solve_wit_17_aux := 
+forall (t2_pre: Z) (t1_pre: Z) (term2: term) (term1: term) (qt2: quant_type) (qv2: (@list Z)) (qterm2: term) (qt1: quant_type) (qv1: (@list Z)) (qterm1: term) (retval: Z) (str: (@list Z)) (retval_2: Z) (z2: Z) (z1: Z) (y2: Z) (y1: Z) (qt2_2: quant_type) (qv2_2: (@list Z)) (qterm2_2: term) (qt1_2: quant_type) (qv1_2: (@list Z)) (qterm1_2: term) (retval_3: Z) (retval_4: Z) (retval_5: Z) ,
+  [| (retval_5 <> 0) |] 
+  &&  [| (retval_4 = retval_3) |] 
+  &&  [| (retval_3 <> 0) |] 
+  &&  [| (t1_pre <> 0) |] 
+  &&  [| (t2_pre <> 0) |] 
+  &&  [| (term1 = (TermQuant (qt1_2) (qv1_2) (qterm1_2))) |] 
+  &&  [| (term2 = (TermQuant (qt2_2) (qv2_2) (qterm2_2))) |] 
+  &&  [| (term_not_contain_var term1 str ) |] 
+  &&  [| (term_not_contain_var term2 str ) |] 
+  &&  [| (retval <> 0) |] 
+  &&  [| (retval = (list_Z_cmp (qv1) (qv2))) |] 
+  &&  [| ((qtID (qt1)) = (qtID (qt2))) |] 
+  &&  [| (t1_pre <> 0) |] 
+  &&  [| (t2_pre <> 0) |] 
+  &&  [| (term1 = (TermQuant (qt1) (qv1) (qterm1))) |] 
+  &&  [| (term2 = (TermQuant (qt2) (qv2) (qterm2))) |] 
+  &&  [| ((termtypeID (term1)) = (termtypeID (term2))) |] 
+  &&  [| (t1_pre <> 0) |] 
+  &&  [| (t2_pre <> 0) |] 
+  &&  [| (t2_pre <> 0) |] 
+  &&  [| (t1_pre <> 0) |] 
+  &&  [| ((termtypeID (term1)) <> 0) |] 
+  &&  [| ((termtypeID (term1)) <> 1) |] 
+  &&  [| ((termtypeID (term1)) <> 2) |] 
+  &&  [| ((termtypeID (term1)) = 3) |]
+  &&  (store_term z2 qterm2_2 )
+  **  (store_term retval_5 qterm2_2 )
+  **  (store_term retval_3 (term_subst_v (str) (qv1_2) (qterm1_2)) )
+  **  (store_string retval_2 str )
+  **  (store_string y1 qv1_2 )
+  **  (store_term z1 qterm1_2 )
+  **  ((&((t1_pre)  # "term" ->ₛ "type")) # Int  |-> (termtypeID (term1)))
+  **  ((&((t2_pre)  # "term" ->ₛ "type")) # Int  |-> (termtypeID (term2)))
+  **  ((&((t1_pre)  # "term" ->ₛ "content" .ₛ "Quant" .ₛ "type")) # Int  |-> (qtID (qt1_2)))
+  **  ((&((t2_pre)  # "term" ->ₛ "content" .ₛ "Quant" .ₛ "type")) # Int  |-> (qtID (qt2_2)))
+  **  ((&((t1_pre)  # "term" ->ₛ "content" .ₛ "Quant" .ₛ "var")) # Ptr  |-> y1)
+  **  ((&((t2_pre)  # "term" ->ₛ "content" .ₛ "Quant" .ₛ "var")) # Ptr  |-> y2)
+  **  ((&((t1_pre)  # "term" ->ₛ "content" .ₛ "Quant" .ₛ "body")) # Ptr  |-> z1)
+  **  ((&((t2_pre)  # "term" ->ₛ "content" .ₛ "Quant" .ₛ "body")) # Ptr  |-> z2)
+  **  (store_string y2 qv2_2 )
+|--
+  [| (retval_5 <> 0) |] 
+  &&  [| (y2 <> 0) |] 
+  &&  [| (retval_2 <> 0) |] 
+  &&  [| (retval_5 <> 0) |] 
+  &&  [| (retval_4 = retval_3) |] 
+  &&  [| (retval_3 <> 0) |] 
+  &&  [| (t1_pre <> 0) |] 
+  &&  [| (t2_pre <> 0) |] 
+  &&  [| (term1 = (TermQuant (qt1_2) (qv1_2) (qterm1_2))) |] 
+  &&  [| (term2 = (TermQuant (qt2_2) (qv2_2) (qterm2_2))) |] 
+  &&  [| (term_not_contain_var term1 str ) |] 
+  &&  [| (term_not_contain_var term2 str ) |] 
+  &&  [| (retval <> 0) |] 
+  &&  [| (retval = (list_Z_cmp (qv1) (qv2))) |] 
+  &&  [| ((qtID (qt1)) = (qtID (qt2))) |] 
+  &&  [| (t1_pre <> 0) |] 
+  &&  [| (t2_pre <> 0) |] 
+  &&  [| (term1 = (TermQuant (qt1) (qv1) (qterm1))) |] 
+  &&  [| (term2 = (TermQuant (qt2) (qv2) (qterm2))) |] 
+  &&  [| ((termtypeID (term1)) = (termtypeID (term2))) |] 
+  &&  [| (t1_pre <> 0) |] 
+  &&  [| (t2_pre <> 0) |] 
+  &&  [| (t2_pre <> 0) |] 
+  &&  [| (t1_pre <> 0) |] 
+  &&  [| ((termtypeID (term1)) <> 0) |] 
+  &&  [| ((termtypeID (term1)) <> 1) |] 
+  &&  [| ((termtypeID (term1)) <> 2) |] 
+  &&  [| ((termtypeID (term1)) = 3) |]
+  &&  (store_term retval_5 qterm2_2 )
+  **  (store_string y2 qv2_2 )
+  **  (store_string retval_2 str )
+  **  (store_term z2 qterm2_2 )
+  **  (store_term retval_3 (term_subst_v (str) (qv1_2) (qterm1_2)) )
+  **  (store_string y1 qv1_2 )
+  **  (store_term z1 qterm1_2 )
+  **  ((&((t1_pre)  # "term" ->ₛ "type")) # Int  |-> (termtypeID (term1)))
+  **  ((&((t2_pre)  # "term" ->ₛ "type")) # Int  |-> (termtypeID (term2)))
+  **  ((&((t1_pre)  # "term" ->ₛ "content" .ₛ "Quant" .ₛ "type")) # Int  |-> (qtID (qt1_2)))
+  **  ((&((t2_pre)  # "term" ->ₛ "content" .ₛ "Quant" .ₛ "type")) # Int  |-> (qtID (qt2_2)))
+  **  ((&((t1_pre)  # "term" ->ₛ "content" .ₛ "Quant" .ₛ "var")) # Ptr  |-> y1)
+  **  ((&((t2_pre)  # "term" ->ₛ "content" .ₛ "Quant" .ₛ "var")) # Ptr  |-> y2)
+  **  ((&((t1_pre)  # "term" ->ₛ "content" .ₛ "Quant" .ₛ "body")) # Ptr  |-> z1)
+  **  ((&((t2_pre)  # "term" ->ₛ "content" .ₛ "Quant" .ₛ "body")) # Ptr  |-> z2)
+.
+
+Definition alpha_equiv_partial_solve_wit_17 := alpha_equiv_partial_solve_wit_17_pure -> alpha_equiv_partial_solve_wit_17_aux.
+
+Definition alpha_equiv_partial_solve_wit_18 := 
+forall (t2_pre: Z) (t1_pre: Z) (term2: term) (term1: term) (qt2: quant_type) (qv2: (@list Z)) (qterm2: term) (qt1: quant_type) (qv1: (@list Z)) (qterm1: term) (retval: Z) (str: (@list Z)) (retval_2: Z) (z2: Z) (z1: Z) (y2: Z) (y1: Z) (qt2_2: quant_type) (qv2_2: (@list Z)) (qterm2_2: term) (qt1_2: quant_type) (qv1_2: (@list Z)) (qterm1_2: term) (retval_3: Z) (retval_4: Z) (retval_5: Z) (retval_6: Z) ,
+  [| (retval_6 = retval_5) |] 
+  &&  [| (retval_5 <> 0) |] 
+  &&  [| (retval_4 = retval_3) |] 
+  &&  [| (retval_3 <> 0) |] 
+  &&  [| (t1_pre <> 0) |] 
+  &&  [| (t2_pre <> 0) |] 
+  &&  [| (term1 = (TermQuant (qt1_2) (qv1_2) (qterm1_2))) |] 
+  &&  [| (term2 = (TermQuant (qt2_2) (qv2_2) (qterm2_2))) |] 
+  &&  [| (term_not_contain_var term1 str ) |] 
+  &&  [| (term_not_contain_var term2 str ) |] 
+  &&  [| (retval <> 0) |] 
+  &&  [| (retval = (list_Z_cmp (qv1) (qv2))) |] 
+  &&  [| ((qtID (qt1)) = (qtID (qt2))) |] 
+  &&  [| (t1_pre <> 0) |] 
+  &&  [| (t2_pre <> 0) |] 
+  &&  [| (term1 = (TermQuant (qt1) (qv1) (qterm1))) |] 
+  &&  [| (term2 = (TermQuant (qt2) (qv2) (qterm2))) |] 
+  &&  [| ((termtypeID (term1)) = (termtypeID (term2))) |] 
+  &&  [| (t1_pre <> 0) |] 
+  &&  [| (t2_pre <> 0) |] 
+  &&  [| (t2_pre <> 0) |] 
+  &&  [| (t1_pre <> 0) |] 
+  &&  [| ((termtypeID (term1)) <> 0) |] 
+  &&  [| ((termtypeID (term1)) <> 1) |] 
+  &&  [| ((termtypeID (term1)) <> 2) |] 
+  &&  [| ((termtypeID (term1)) = 3) |]
+  &&  (store_term retval_5 (term_subst_v (str) (qv2_2) (qterm2_2)) )
+  **  (store_string retval_2 str )
+  **  (store_string y2 qv2_2 )
+  **  (store_term z2 qterm2_2 )
+  **  (store_term retval_3 (term_subst_v (str) (qv1_2) (qterm1_2)) )
+  **  (store_string y1 qv1_2 )
+  **  (store_term z1 qterm1_2 )
+  **  ((&((t1_pre)  # "term" ->ₛ "type")) # Int  |-> (termtypeID (term1)))
+  **  ((&((t2_pre)  # "term" ->ₛ "type")) # Int  |-> (termtypeID (term2)))
+  **  ((&((t1_pre)  # "term" ->ₛ "content" .ₛ "Quant" .ₛ "type")) # Int  |-> (qtID (qt1_2)))
+  **  ((&((t2_pre)  # "term" ->ₛ "content" .ₛ "Quant" .ₛ "type")) # Int  |-> (qtID (qt2_2)))
+  **  ((&((t1_pre)  # "term" ->ₛ "content" .ₛ "Quant" .ₛ "var")) # Ptr  |-> y1)
+  **  ((&((t2_pre)  # "term" ->ₛ "content" .ₛ "Quant" .ₛ "var")) # Ptr  |-> y2)
+  **  ((&((t1_pre)  # "term" ->ₛ "content" .ₛ "Quant" .ₛ "body")) # Ptr  |-> z1)
+  **  ((&((t2_pre)  # "term" ->ₛ "content" .ₛ "Quant" .ₛ "body")) # Ptr  |-> z2)
+|--
+  [| (retval_6 = retval_5) |] 
+  &&  [| (retval_5 <> 0) |] 
+  &&  [| (retval_4 = retval_3) |] 
+  &&  [| (retval_3 <> 0) |] 
+  &&  [| (t1_pre <> 0) |] 
+  &&  [| (t2_pre <> 0) |] 
+  &&  [| (term1 = (TermQuant (qt1_2) (qv1_2) (qterm1_2))) |] 
+  &&  [| (term2 = (TermQuant (qt2_2) (qv2_2) (qterm2_2))) |] 
+  &&  [| (term_not_contain_var term1 str ) |] 
+  &&  [| (term_not_contain_var term2 str ) |] 
+  &&  [| (retval <> 0) |] 
+  &&  [| (retval = (list_Z_cmp (qv1) (qv2))) |] 
+  &&  [| ((qtID (qt1)) = (qtID (qt2))) |] 
+  &&  [| (t1_pre <> 0) |] 
+  &&  [| (t2_pre <> 0) |] 
+  &&  [| (term1 = (TermQuant (qt1) (qv1) (qterm1))) |] 
+  &&  [| (term2 = (TermQuant (qt2) (qv2) (qterm2))) |] 
+  &&  [| ((termtypeID (term1)) = (termtypeID (term2))) |] 
+  &&  [| (t1_pre <> 0) |] 
+  &&  [| (t2_pre <> 0) |] 
+  &&  [| (t2_pre <> 0) |] 
+  &&  [| (t1_pre <> 0) |] 
+  &&  [| ((termtypeID (term1)) <> 0) |] 
+  &&  [| ((termtypeID (term1)) <> 1) |] 
+  &&  [| ((termtypeID (term1)) <> 2) |] 
+  &&  [| ((termtypeID (term1)) = 3) |]
+  &&  (store_term retval_4 (term_subst_v (str) (qv1_2) (qterm1_2)) )
+  **  (store_term retval_6 (term_subst_v (str) (qv2_2) (qterm2_2)) )
+  **  (store_string retval_2 str )
+  **  (store_string y2 qv2_2 )
+  **  (store_term z2 qterm2_2 )
+  **  (store_string y1 qv1_2 )
+  **  (store_term z1 qterm1_2 )
+  **  ((&((t1_pre)  # "term" ->ₛ "type")) # Int  |-> (termtypeID (term1)))
+  **  ((&((t2_pre)  # "term" ->ₛ "type")) # Int  |-> (termtypeID (term2)))
+  **  ((&((t1_pre)  # "term" ->ₛ "content" .ₛ "Quant" .ₛ "type")) # Int  |-> (qtID (qt1_2)))
+  **  ((&((t2_pre)  # "term" ->ₛ "content" .ₛ "Quant" .ₛ "type")) # Int  |-> (qtID (qt2_2)))
+  **  ((&((t1_pre)  # "term" ->ₛ "content" .ₛ "Quant" .ₛ "var")) # Ptr  |-> y1)
+  **  ((&((t2_pre)  # "term" ->ₛ "content" .ₛ "Quant" .ₛ "var")) # Ptr  |-> y2)
+  **  ((&((t1_pre)  # "term" ->ₛ "content" .ₛ "Quant" .ₛ "body")) # Ptr  |-> z1)
+  **  ((&((t2_pre)  # "term" ->ₛ "content" .ₛ "Quant" .ₛ "body")) # Ptr  |-> z2)
+.
+
+Definition alpha_equiv_partial_solve_wit_19 := 
+forall (t2_pre: Z) (t1_pre: Z) (term2: term) (term1: term) (qt2: quant_type) (qv2: (@list Z)) (qterm2: term) (qt1: quant_type) (qv1: (@list Z)) (qterm1: term) (retval: Z) (str: (@list Z)) (retval_2: Z) (z2: Z) (z1: Z) (y2: Z) (y1: Z) (qt2_2: quant_type) (qv2_2: (@list Z)) (qterm2_2: term) (qt1_2: quant_type) (qv1_2: (@list Z)) (qterm1_2: term) (retval_3: Z) (retval_4: Z) (retval_5: Z) (retval_6: Z) (retval_7: Z) ,
+  [| (retval_7 = (term_eqn ((term_subst_v (str) (qv1_2) (qterm1_2))) ((term_subst_v (str) (qv2_2) (qterm2_2))))) |] 
+  &&  [| (retval_6 = retval_5) |] 
+  &&  [| (retval_5 <> 0) |] 
+  &&  [| (retval_4 = retval_3) |] 
+  &&  [| (retval_3 <> 0) |] 
+  &&  [| (t1_pre <> 0) |] 
+  &&  [| (t2_pre <> 0) |] 
+  &&  [| (term1 = (TermQuant (qt1_2) (qv1_2) (qterm1_2))) |] 
+  &&  [| (term2 = (TermQuant (qt2_2) (qv2_2) (qterm2_2))) |] 
+  &&  [| (term_not_contain_var term1 str ) |] 
+  &&  [| (term_not_contain_var term2 str ) |] 
+  &&  [| (retval <> 0) |] 
+  &&  [| (retval = (list_Z_cmp (qv1) (qv2))) |] 
+  &&  [| ((qtID (qt1)) = (qtID (qt2))) |] 
+  &&  [| (t1_pre <> 0) |] 
+  &&  [| (t2_pre <> 0) |] 
+  &&  [| (term1 = (TermQuant (qt1) (qv1) (qterm1))) |] 
+  &&  [| (term2 = (TermQuant (qt2) (qv2) (qterm2))) |] 
+  &&  [| ((termtypeID (term1)) = (termtypeID (term2))) |] 
+  &&  [| (t1_pre <> 0) |] 
+  &&  [| (t2_pre <> 0) |] 
+  &&  [| (t2_pre <> 0) |] 
+  &&  [| (t1_pre <> 0) |] 
+  &&  [| ((termtypeID (term1)) <> 0) |] 
+  &&  [| ((termtypeID (term1)) <> 1) |] 
+  &&  [| ((termtypeID (term1)) <> 2) |] 
+  &&  [| ((termtypeID (term1)) = 3) |]
+  &&  (store_term retval_4 (term_subst_v (str) (qv1_2) (qterm1_2)) )
+  **  (store_term retval_6 (term_subst_v (str) (qv2_2) (qterm2_2)) )
+  **  (store_string retval_2 str )
+  **  (store_string y2 qv2_2 )
+  **  (store_term z2 qterm2_2 )
+  **  (store_string y1 qv1_2 )
+  **  (store_term z1 qterm1_2 )
+  **  ((&((t1_pre)  # "term" ->ₛ "type")) # Int  |-> (termtypeID (term1)))
+  **  ((&((t2_pre)  # "term" ->ₛ "type")) # Int  |-> (termtypeID (term2)))
+  **  ((&((t1_pre)  # "term" ->ₛ "content" .ₛ "Quant" .ₛ "type")) # Int  |-> (qtID (qt1_2)))
+  **  ((&((t2_pre)  # "term" ->ₛ "content" .ₛ "Quant" .ₛ "type")) # Int  |-> (qtID (qt2_2)))
+  **  ((&((t1_pre)  # "term" ->ₛ "content" .ₛ "Quant" .ₛ "var")) # Ptr  |-> y1)
+  **  ((&((t2_pre)  # "term" ->ₛ "content" .ₛ "Quant" .ₛ "var")) # Ptr  |-> y2)
+  **  ((&((t1_pre)  # "term" ->ₛ "content" .ₛ "Quant" .ₛ "body")) # Ptr  |-> z1)
+  **  ((&((t2_pre)  # "term" ->ₛ "content" .ₛ "Quant" .ₛ "body")) # Ptr  |-> z2)
+|--
+  [| (retval_7 = (term_eqn ((term_subst_v (str) (qv1_2) (qterm1_2))) ((term_subst_v (str) (qv2_2) (qterm2_2))))) |] 
+  &&  [| (retval_6 = retval_5) |] 
+  &&  [| (retval_5 <> 0) |] 
+  &&  [| (retval_4 = retval_3) |] 
+  &&  [| (retval_3 <> 0) |] 
+  &&  [| (t1_pre <> 0) |] 
+  &&  [| (t2_pre <> 0) |] 
+  &&  [| (term1 = (TermQuant (qt1_2) (qv1_2) (qterm1_2))) |] 
+  &&  [| (term2 = (TermQuant (qt2_2) (qv2_2) (qterm2_2))) |] 
+  &&  [| (term_not_contain_var term1 str ) |] 
+  &&  [| (term_not_contain_var term2 str ) |] 
+  &&  [| (retval <> 0) |] 
+  &&  [| (retval = (list_Z_cmp (qv1) (qv2))) |] 
+  &&  [| ((qtID (qt1)) = (qtID (qt2))) |] 
+  &&  [| (t1_pre <> 0) |] 
+  &&  [| (t2_pre <> 0) |] 
+  &&  [| (term1 = (TermQuant (qt1) (qv1) (qterm1))) |] 
+  &&  [| (term2 = (TermQuant (qt2) (qv2) (qterm2))) |] 
+  &&  [| ((termtypeID (term1)) = (termtypeID (term2))) |] 
+  &&  [| (t1_pre <> 0) |] 
+  &&  [| (t2_pre <> 0) |] 
+  &&  [| (t2_pre <> 0) |] 
+  &&  [| (t1_pre <> 0) |] 
+  &&  [| ((termtypeID (term1)) <> 0) |] 
+  &&  [| ((termtypeID (term1)) <> 1) |] 
+  &&  [| ((termtypeID (term1)) <> 2) |] 
+  &&  [| ((termtypeID (term1)) = 3) |]
+  &&  (store_term retval_4 (term_subst_v (str) (qv1_2) (qterm1_2)) )
+  **  (store_term retval_6 (term_subst_v (str) (qv2_2) (qterm2_2)) )
+  **  (store_string retval_2 str )
+  **  (store_string y2 qv2_2 )
+  **  (store_term z2 qterm2_2 )
+  **  (store_string y1 qv1_2 )
+  **  (store_term z1 qterm1_2 )
+  **  ((&((t1_pre)  # "term" ->ₛ "type")) # Int  |-> (termtypeID (term1)))
+  **  ((&((t2_pre)  # "term" ->ₛ "type")) # Int  |-> (termtypeID (term2)))
+  **  ((&((t1_pre)  # "term" ->ₛ "content" .ₛ "Quant" .ₛ "type")) # Int  |-> (qtID (qt1_2)))
+  **  ((&((t2_pre)  # "term" ->ₛ "content" .ₛ "Quant" .ₛ "type")) # Int  |-> (qtID (qt2_2)))
+  **  ((&((t1_pre)  # "term" ->ₛ "content" .ₛ "Quant" .ₛ "var")) # Ptr  |-> y1)
+  **  ((&((t2_pre)  # "term" ->ₛ "content" .ₛ "Quant" .ₛ "var")) # Ptr  |-> y2)
+  **  ((&((t1_pre)  # "term" ->ₛ "content" .ₛ "Quant" .ₛ "body")) # Ptr  |-> z1)
+  **  ((&((t2_pre)  # "term" ->ₛ "content" .ₛ "Quant" .ₛ "body")) # Ptr  |-> z2)
+.
+
+Definition alpha_equiv_partial_solve_wit_20 := 
+forall (t2_pre: Z) (t1_pre: Z) (term2: term) (term1: term) (qt2: quant_type) (qv2: (@list Z)) (qterm2: term) (qt1: quant_type) (qv1: (@list Z)) (qterm1: term) (retval: Z) (str: (@list Z)) (retval_2: Z) (z2: Z) (z1: Z) (y2: Z) (y1: Z) (qt2_2: quant_type) (qv2_2: (@list Z)) (qterm2_2: term) (qt1_2: quant_type) (qv1_2: (@list Z)) (qterm1_2: term) (retval_3: Z) (retval_4: Z) (retval_5: Z) (retval_6: Z) (retval_7: Z) ,
+  [| (retval_7 = (term_eqn ((term_subst_v (str) (qv1_2) (qterm1_2))) ((term_subst_v (str) (qv2_2) (qterm2_2))))) |] 
+  &&  [| (retval_6 = retval_5) |] 
+  &&  [| (retval_5 <> 0) |] 
+  &&  [| (retval_4 = retval_3) |] 
+  &&  [| (retval_3 <> 0) |] 
+  &&  [| (t1_pre <> 0) |] 
+  &&  [| (t2_pre <> 0) |] 
+  &&  [| (term1 = (TermQuant (qt1_2) (qv1_2) (qterm1_2))) |] 
+  &&  [| (term2 = (TermQuant (qt2_2) (qv2_2) (qterm2_2))) |] 
+  &&  [| (term_not_contain_var term1 str ) |] 
+  &&  [| (term_not_contain_var term2 str ) |] 
+  &&  [| (retval <> 0) |] 
+  &&  [| (retval = (list_Z_cmp (qv1) (qv2))) |] 
+  &&  [| ((qtID (qt1)) = (qtID (qt2))) |] 
+  &&  [| (t1_pre <> 0) |] 
+  &&  [| (t2_pre <> 0) |] 
+  &&  [| (term1 = (TermQuant (qt1) (qv1) (qterm1))) |] 
+  &&  [| (term2 = (TermQuant (qt2) (qv2) (qterm2))) |] 
+  &&  [| ((termtypeID (term1)) = (termtypeID (term2))) |] 
+  &&  [| (t1_pre <> 0) |] 
+  &&  [| (t2_pre <> 0) |] 
+  &&  [| (t2_pre <> 0) |] 
+  &&  [| (t1_pre <> 0) |] 
+  &&  [| ((termtypeID (term1)) <> 0) |] 
+  &&  [| ((termtypeID (term1)) <> 1) |] 
+  &&  [| ((termtypeID (term1)) <> 2) |] 
+  &&  [| ((termtypeID (term1)) = 3) |]
+  &&  (store_term retval_6 (term_subst_v (str) (qv2_2) (qterm2_2)) )
+  **  (store_string retval_2 str )
+  **  (store_string y2 qv2_2 )
+  **  (store_term z2 qterm2_2 )
+  **  (store_string y1 qv1_2 )
+  **  (store_term z1 qterm1_2 )
+  **  ((&((t1_pre)  # "term" ->ₛ "type")) # Int  |-> (termtypeID (term1)))
+  **  ((&((t2_pre)  # "term" ->ₛ "type")) # Int  |-> (termtypeID (term2)))
+  **  ((&((t1_pre)  # "term" ->ₛ "content" .ₛ "Quant" .ₛ "type")) # Int  |-> (qtID (qt1_2)))
+  **  ((&((t2_pre)  # "term" ->ₛ "content" .ₛ "Quant" .ₛ "type")) # Int  |-> (qtID (qt2_2)))
+  **  ((&((t1_pre)  # "term" ->ₛ "content" .ₛ "Quant" .ₛ "var")) # Ptr  |-> y1)
+  **  ((&((t2_pre)  # "term" ->ₛ "content" .ₛ "Quant" .ₛ "var")) # Ptr  |-> y2)
+  **  ((&((t1_pre)  # "term" ->ₛ "content" .ₛ "Quant" .ₛ "body")) # Ptr  |-> z1)
+  **  ((&((t2_pre)  # "term" ->ₛ "content" .ₛ "Quant" .ₛ "body")) # Ptr  |-> z2)
+|--
+  [| (retval_7 = (term_eqn ((term_subst_v (str) (qv1_2) (qterm1_2))) ((term_subst_v (str) (qv2_2) (qterm2_2))))) |] 
+  &&  [| (retval_6 = retval_5) |] 
+  &&  [| (retval_5 <> 0) |] 
+  &&  [| (retval_4 = retval_3) |] 
+  &&  [| (retval_3 <> 0) |] 
+  &&  [| (t1_pre <> 0) |] 
+  &&  [| (t2_pre <> 0) |] 
+  &&  [| (term1 = (TermQuant (qt1_2) (qv1_2) (qterm1_2))) |] 
+  &&  [| (term2 = (TermQuant (qt2_2) (qv2_2) (qterm2_2))) |] 
+  &&  [| (term_not_contain_var term1 str ) |] 
+  &&  [| (term_not_contain_var term2 str ) |] 
+  &&  [| (retval <> 0) |] 
+  &&  [| (retval = (list_Z_cmp (qv1) (qv2))) |] 
+  &&  [| ((qtID (qt1)) = (qtID (qt2))) |] 
+  &&  [| (t1_pre <> 0) |] 
+  &&  [| (t2_pre <> 0) |] 
+  &&  [| (term1 = (TermQuant (qt1) (qv1) (qterm1))) |] 
+  &&  [| (term2 = (TermQuant (qt2) (qv2) (qterm2))) |] 
+  &&  [| ((termtypeID (term1)) = (termtypeID (term2))) |] 
+  &&  [| (t1_pre <> 0) |] 
+  &&  [| (t2_pre <> 0) |] 
+  &&  [| (t2_pre <> 0) |] 
+  &&  [| (t1_pre <> 0) |] 
+  &&  [| ((termtypeID (term1)) <> 0) |] 
+  &&  [| ((termtypeID (term1)) <> 1) |] 
+  &&  [| ((termtypeID (term1)) <> 2) |] 
+  &&  [| ((termtypeID (term1)) = 3) |]
+  &&  (store_term retval_6 (term_subst_v (str) (qv2_2) (qterm2_2)) )
+  **  (store_string retval_2 str )
+  **  (store_string y2 qv2_2 )
+  **  (store_term z2 qterm2_2 )
+  **  (store_string y1 qv1_2 )
+  **  (store_term z1 qterm1_2 )
+  **  ((&((t1_pre)  # "term" ->ₛ "type")) # Int  |-> (termtypeID (term1)))
+  **  ((&((t2_pre)  # "term" ->ₛ "type")) # Int  |-> (termtypeID (term2)))
+  **  ((&((t1_pre)  # "term" ->ₛ "content" .ₛ "Quant" .ₛ "type")) # Int  |-> (qtID (qt1_2)))
+  **  ((&((t2_pre)  # "term" ->ₛ "content" .ₛ "Quant" .ₛ "type")) # Int  |-> (qtID (qt2_2)))
+  **  ((&((t1_pre)  # "term" ->ₛ "content" .ₛ "Quant" .ₛ "var")) # Ptr  |-> y1)
+  **  ((&((t2_pre)  # "term" ->ₛ "content" .ₛ "Quant" .ₛ "var")) # Ptr  |-> y2)
+  **  ((&((t1_pre)  # "term" ->ₛ "content" .ₛ "Quant" .ₛ "body")) # Ptr  |-> z1)
+  **  ((&((t2_pre)  # "term" ->ₛ "content" .ₛ "Quant" .ₛ "body")) # Ptr  |-> z2)
+.
+
+Definition alpha_equiv_partial_solve_wit_21_pure := 
+forall (t2_pre: Z) (t1_pre: Z) (term2: term) (term1: term) (qt2: quant_type) (qv2: (@list Z)) (qterm2: term) (qt1: quant_type) (qv1: (@list Z)) (qterm1: term) (retval_2: Z) (str: (@list Z)) (retval: Z) (z2: Z) (z1: Z) (y2: Z) (y1: Z) (qt2_2: quant_type) (qv2_2: (@list Z)) (qterm2_2: term) (qt1_2: quant_type) (qv1_2: (@list Z)) (qterm1_2: term) (retval_3: Z) (retval_4: Z) (retval_5: Z) (retval_6: Z) (retval_7: Z) ,
+  [| (retval_7 = (term_eqn ((term_subst_v (str) (qv1_2) (qterm1_2))) ((term_subst_v (str) (qv2_2) (qterm2_2))))) |] 
+  &&  [| (retval_6 = retval_5) |] 
+  &&  [| (retval_5 <> 0) |] 
+  &&  [| (retval_4 = retval_3) |] 
+  &&  [| (retval_3 <> 0) |] 
+  &&  [| (t1_pre <> 0) |] 
+  &&  [| (t2_pre <> 0) |] 
+  &&  [| (term1 = (TermQuant (qt1_2) (qv1_2) (qterm1_2))) |] 
+  &&  [| (term2 = (TermQuant (qt2_2) (qv2_2) (qterm2_2))) |] 
+  &&  [| (term_not_contain_var term1 str ) |] 
+  &&  [| (term_not_contain_var term2 str ) |] 
   &&  [| (retval_2 <> 0) |] 
   &&  [| (retval_2 = (list_Z_cmp (qv1) (qv2))) |] 
   &&  [| ((qtID (qt1)) = (qtID (qt2))) |] 
@@ -1423,33 +2201,84 @@ forall (t2_pre: Z) (t1_pre: Z) (term2: term) (term1: term) (z2: Z) (z1: Z) (y2: 
   &&  [| ((termtypeID (term1)) <> 1) |] 
   &&  [| ((termtypeID (term1)) <> 2) |] 
   &&  [| ((termtypeID (term1)) = 3) |]
-  &&  (store_term z2 qterm2 )
-  **  (store_term retval qterm2 )
-  **  ((( &( "t21" ) )) # Ptr  |->_)
+  &&  ((( &( "result" ) )) # Int  |-> retval_7)
+  **  (store_string retval str )
+  **  (store_string y2 qv2_2 )
+  **  (store_term z2 qterm2_2 )
+  **  ((( &( "new_t2" ) )) # Ptr  |-> retval_6)
+  **  (store_string y1 qv1_2 )
+  **  (store_term z1 qterm1_2 )
+  **  ((( &( "new_t1" ) )) # Ptr  |-> retval_4)
   **  ((( &( "t1" ) )) # Ptr  |-> t1_pre)
-  **  ((&((t1_pre)  # "term" ->ₛ "content" .ₛ "Quant" .ₛ "var")) # Ptr  |-> y1)
   **  ((( &( "t2" ) )) # Ptr  |-> t2_pre)
-  **  ((&((t2_pre)  # "term" ->ₛ "content" .ₛ "Quant" .ₛ "var")) # Ptr  |-> y2)
-  **  (store_string y1 qv1 )
-  **  (store_string y2 qv2 )
   **  ((&((t1_pre)  # "term" ->ₛ "type")) # Int  |-> (termtypeID (term1)))
   **  ((&((t2_pre)  # "term" ->ₛ "type")) # Int  |-> (termtypeID (term2)))
-  **  ((&((t1_pre)  # "term" ->ₛ "content" .ₛ "Quant" .ₛ "type")) # Int  |-> (qtID (qt1)))
-  **  ((&((t2_pre)  # "term" ->ₛ "content" .ₛ "Quant" .ₛ "type")) # Int  |-> (qtID (qt2)))
+  **  ((&((t1_pre)  # "term" ->ₛ "content" .ₛ "Quant" .ₛ "type")) # Int  |-> (qtID (qt1_2)))
+  **  ((&((t2_pre)  # "term" ->ₛ "content" .ₛ "Quant" .ₛ "type")) # Int  |-> (qtID (qt2_2)))
+  **  ((&((t1_pre)  # "term" ->ₛ "content" .ₛ "Quant" .ₛ "var")) # Ptr  |-> y1)
+  **  ((&((t2_pre)  # "term" ->ₛ "content" .ₛ "Quant" .ₛ "var")) # Ptr  |-> y2)
   **  ((&((t1_pre)  # "term" ->ₛ "content" .ₛ "Quant" .ₛ "body")) # Ptr  |-> z1)
   **  ((&((t2_pre)  # "term" ->ₛ "content" .ₛ "Quant" .ₛ "body")) # Ptr  |-> z2)
-  **  (store_term z1 qterm1 )
+  **  ((( &( "new_var" ) )) # Ptr  |-> retval)
 |--
-  [| (y1 <> 0) |] 
-  &&  [| (y2 <> 0) |] 
-  &&  [| (retval <> 0) |]
+  [| (retval <> 0) |]
 .
 
-Definition alpha_equiv_partial_solve_wit_13_aux := 
-forall (t2_pre: Z) (t1_pre: Z) (term2: term) (term1: term) (z2: Z) (z1: Z) (y2: Z) (y1: Z) (qt2: quant_type) (qv2: (@list Z)) (qterm2: term) (qt1: quant_type) (qv1: (@list Z)) (qterm1: term) (retval: Z) (retval_2: Z) ,
+Definition alpha_equiv_partial_solve_wit_21_aux := 
+forall (t2_pre: Z) (t1_pre: Z) (term2: term) (term1: term) (qt2: quant_type) (qv2: (@list Z)) (qterm2: term) (qt1: quant_type) (qv1: (@list Z)) (qterm1: term) (retval: Z) (str: (@list Z)) (retval_2: Z) (z2: Z) (z1: Z) (y2: Z) (y1: Z) (qt2_2: quant_type) (qv2_2: (@list Z)) (qterm2_2: term) (qt1_2: quant_type) (qv1_2: (@list Z)) (qterm1_2: term) (retval_3: Z) (retval_4: Z) (retval_5: Z) (retval_6: Z) (retval_7: Z) ,
+  [| (retval_7 = (term_eqn ((term_subst_v (str) (qv1_2) (qterm1_2))) ((term_subst_v (str) (qv2_2) (qterm2_2))))) |] 
+  &&  [| (retval_6 = retval_5) |] 
+  &&  [| (retval_5 <> 0) |] 
+  &&  [| (retval_4 = retval_3) |] 
+  &&  [| (retval_3 <> 0) |] 
+  &&  [| (t1_pre <> 0) |] 
+  &&  [| (t2_pre <> 0) |] 
+  &&  [| (term1 = (TermQuant (qt1_2) (qv1_2) (qterm1_2))) |] 
+  &&  [| (term2 = (TermQuant (qt2_2) (qv2_2) (qterm2_2))) |] 
+  &&  [| (term_not_contain_var term1 str ) |] 
+  &&  [| (term_not_contain_var term2 str ) |] 
+  &&  [| (retval <> 0) |] 
+  &&  [| (retval = (list_Z_cmp (qv1) (qv2))) |] 
+  &&  [| ((qtID (qt1)) = (qtID (qt2))) |] 
+  &&  [| (t1_pre <> 0) |] 
+  &&  [| (t2_pre <> 0) |] 
+  &&  [| (term1 = (TermQuant (qt1) (qv1) (qterm1))) |] 
+  &&  [| (term2 = (TermQuant (qt2) (qv2) (qterm2))) |] 
+  &&  [| ((termtypeID (term1)) = (termtypeID (term2))) |] 
+  &&  [| (t1_pre <> 0) |] 
+  &&  [| (t2_pre <> 0) |] 
+  &&  [| (t2_pre <> 0) |] 
+  &&  [| (t1_pre <> 0) |] 
+  &&  [| ((termtypeID (term1)) <> 0) |] 
+  &&  [| ((termtypeID (term1)) <> 1) |] 
+  &&  [| ((termtypeID (term1)) <> 2) |] 
+  &&  [| ((termtypeID (term1)) = 3) |]
+  &&  (store_string retval_2 str )
+  **  (store_string y2 qv2_2 )
+  **  (store_term z2 qterm2_2 )
+  **  (store_string y1 qv1_2 )
+  **  (store_term z1 qterm1_2 )
+  **  ((&((t1_pre)  # "term" ->ₛ "type")) # Int  |-> (termtypeID (term1)))
+  **  ((&((t2_pre)  # "term" ->ₛ "type")) # Int  |-> (termtypeID (term2)))
+  **  ((&((t1_pre)  # "term" ->ₛ "content" .ₛ "Quant" .ₛ "type")) # Int  |-> (qtID (qt1_2)))
+  **  ((&((t2_pre)  # "term" ->ₛ "content" .ₛ "Quant" .ₛ "type")) # Int  |-> (qtID (qt2_2)))
+  **  ((&((t1_pre)  # "term" ->ₛ "content" .ₛ "Quant" .ₛ "var")) # Ptr  |-> y1)
+  **  ((&((t2_pre)  # "term" ->ₛ "content" .ₛ "Quant" .ₛ "var")) # Ptr  |-> y2)
+  **  ((&((t1_pre)  # "term" ->ₛ "content" .ₛ "Quant" .ₛ "body")) # Ptr  |-> z1)
+  **  ((&((t2_pre)  # "term" ->ₛ "content" .ₛ "Quant" .ₛ "body")) # Ptr  |-> z2)
+|--
   [| (retval_2 <> 0) |] 
-  &&  [| (y1 <> 0) |] 
-  &&  [| (y2 <> 0) |] 
+  &&  [| (retval_7 = (term_eqn ((term_subst_v (str) (qv1_2) (qterm1_2))) ((term_subst_v (str) (qv2_2) (qterm2_2))))) |] 
+  &&  [| (retval_6 = retval_5) |] 
+  &&  [| (retval_5 <> 0) |] 
+  &&  [| (retval_4 = retval_3) |] 
+  &&  [| (retval_3 <> 0) |] 
+  &&  [| (t1_pre <> 0) |] 
+  &&  [| (t2_pre <> 0) |] 
+  &&  [| (term1 = (TermQuant (qt1_2) (qv1_2) (qterm1_2))) |] 
+  &&  [| (term2 = (TermQuant (qt2_2) (qv2_2) (qterm2_2))) |] 
+  &&  [| (term_not_contain_var term1 str ) |] 
+  &&  [| (term_not_contain_var term2 str ) |] 
   &&  [| (retval <> 0) |] 
   &&  [| (retval = (list_Z_cmp (qv1) (qv2))) |] 
   &&  [| ((qtID (qt1)) = (qtID (qt2))) |] 
@@ -1466,202 +2295,22 @@ forall (t2_pre: Z) (t1_pre: Z) (term2: term) (term1: term) (z2: Z) (z1: Z) (y2: 
   &&  [| ((termtypeID (term1)) <> 1) |] 
   &&  [| ((termtypeID (term1)) <> 2) |] 
   &&  [| ((termtypeID (term1)) = 3) |]
-  &&  (store_term z2 qterm2 )
-  **  (store_term retval_2 qterm2 )
-  **  ((&((t1_pre)  # "term" ->ₛ "content" .ₛ "Quant" .ₛ "var")) # Ptr  |-> y1)
-  **  ((&((t2_pre)  # "term" ->ₛ "content" .ₛ "Quant" .ₛ "var")) # Ptr  |-> y2)
-  **  (store_string y1 qv1 )
-  **  (store_string y2 qv2 )
+  &&  (store_string retval_2 str )
+  **  (store_string y2 qv2_2 )
+  **  (store_term z2 qterm2_2 )
+  **  (store_string y1 qv1_2 )
+  **  (store_term z1 qterm1_2 )
   **  ((&((t1_pre)  # "term" ->ₛ "type")) # Int  |-> (termtypeID (term1)))
   **  ((&((t2_pre)  # "term" ->ₛ "type")) # Int  |-> (termtypeID (term2)))
-  **  ((&((t1_pre)  # "term" ->ₛ "content" .ₛ "Quant" .ₛ "type")) # Int  |-> (qtID (qt1)))
-  **  ((&((t2_pre)  # "term" ->ₛ "content" .ₛ "Quant" .ₛ "type")) # Int  |-> (qtID (qt2)))
-  **  ((&((t1_pre)  # "term" ->ₛ "content" .ₛ "Quant" .ₛ "body")) # Ptr  |-> z1)
-  **  ((&((t2_pre)  # "term" ->ₛ "content" .ₛ "Quant" .ₛ "body")) # Ptr  |-> z2)
-  **  (store_term z1 qterm1 )
-|--
-  [| (y1 <> 0) |] 
-  &&  [| (y2 <> 0) |] 
-  &&  [| (retval_2 <> 0) |] 
-  &&  [| (retval_2 <> 0) |] 
-  &&  [| (y1 <> 0) |] 
-  &&  [| (y2 <> 0) |] 
-  &&  [| (retval <> 0) |] 
-  &&  [| (retval = (list_Z_cmp (qv1) (qv2))) |] 
-  &&  [| ((qtID (qt1)) = (qtID (qt2))) |] 
-  &&  [| (t1_pre <> 0) |] 
-  &&  [| (t2_pre <> 0) |] 
-  &&  [| (term1 = (TermQuant (qt1) (qv1) (qterm1))) |] 
-  &&  [| (term2 = (TermQuant (qt2) (qv2) (qterm2))) |] 
-  &&  [| ((termtypeID (term1)) = (termtypeID (term2))) |] 
-  &&  [| (t1_pre <> 0) |] 
-  &&  [| (t2_pre <> 0) |] 
-  &&  [| (t2_pre <> 0) |] 
-  &&  [| (t1_pre <> 0) |] 
-  &&  [| ((termtypeID (term1)) <> 0) |] 
-  &&  [| ((termtypeID (term1)) <> 1) |] 
-  &&  [| ((termtypeID (term1)) <> 2) |] 
-  &&  [| ((termtypeID (term1)) = 3) |]
-  &&  (store_term retval_2 qterm2 )
-  **  (store_string y2 qv2 )
-  **  (store_string y1 qv1 )
-  **  (store_term z2 qterm2 )
+  **  ((&((t1_pre)  # "term" ->ₛ "content" .ₛ "Quant" .ₛ "type")) # Int  |-> (qtID (qt1_2)))
+  **  ((&((t2_pre)  # "term" ->ₛ "content" .ₛ "Quant" .ₛ "type")) # Int  |-> (qtID (qt2_2)))
   **  ((&((t1_pre)  # "term" ->ₛ "content" .ₛ "Quant" .ₛ "var")) # Ptr  |-> y1)
   **  ((&((t2_pre)  # "term" ->ₛ "content" .ₛ "Quant" .ₛ "var")) # Ptr  |-> y2)
-  **  ((&((t1_pre)  # "term" ->ₛ "type")) # Int  |-> (termtypeID (term1)))
-  **  ((&((t2_pre)  # "term" ->ₛ "type")) # Int  |-> (termtypeID (term2)))
-  **  ((&((t1_pre)  # "term" ->ₛ "content" .ₛ "Quant" .ₛ "type")) # Int  |-> (qtID (qt1)))
-  **  ((&((t2_pre)  # "term" ->ₛ "content" .ₛ "Quant" .ₛ "type")) # Int  |-> (qtID (qt2)))
-  **  ((&((t1_pre)  # "term" ->ₛ "content" .ₛ "Quant" .ₛ "body")) # Ptr  |-> z1)
-  **  ((&((t2_pre)  # "term" ->ₛ "content" .ₛ "Quant" .ₛ "body")) # Ptr  |-> z2)
-  **  (store_term z1 qterm1 )
-.
-
-Definition alpha_equiv_partial_solve_wit_13 := alpha_equiv_partial_solve_wit_13_pure -> alpha_equiv_partial_solve_wit_13_aux.
-
-Definition alpha_equiv_partial_solve_wit_14 := 
-forall (t2_pre: Z) (t1_pre: Z) (term2: term) (term1: term) (z2: Z) (z1: Z) (y2: Z) (y1: Z) (qt2: quant_type) (qv2: (@list Z)) (qterm2: term) (qt1: quant_type) (qv1: (@list Z)) (qterm1: term) (retval: Z) (retval_2: Z) (retval_3: Z) ,
-  [| (retval_3 = retval_2) |] 
-  &&  [| (retval_2 <> 0) |] 
-  &&  [| (y1 <> 0) |] 
-  &&  [| (y2 <> 0) |] 
-  &&  [| (retval <> 0) |] 
-  &&  [| (retval = (list_Z_cmp (qv1) (qv2))) |] 
-  &&  [| ((qtID (qt1)) = (qtID (qt2))) |] 
-  &&  [| (t1_pre <> 0) |] 
-  &&  [| (t2_pre <> 0) |] 
-  &&  [| (term1 = (TermQuant (qt1) (qv1) (qterm1))) |] 
-  &&  [| (term2 = (TermQuant (qt2) (qv2) (qterm2))) |] 
-  &&  [| ((termtypeID (term1)) = (termtypeID (term2))) |] 
-  &&  [| (t1_pre <> 0) |] 
-  &&  [| (t2_pre <> 0) |] 
-  &&  [| (t2_pre <> 0) |] 
-  &&  [| (t1_pre <> 0) |] 
-  &&  [| ((termtypeID (term1)) <> 0) |] 
-  &&  [| ((termtypeID (term1)) <> 1) |] 
-  &&  [| ((termtypeID (term1)) <> 2) |] 
-  &&  [| ((termtypeID (term1)) = 3) |]
-  &&  (store_term retval_2 (term_subst_v (qv1) (qv2) (qterm2)) )
-  **  (store_string y1 qv1 )
-  **  (store_string y2 qv2 )
-  **  (store_term z2 qterm2 )
-  **  ((&((t1_pre)  # "term" ->ₛ "content" .ₛ "Quant" .ₛ "var")) # Ptr  |-> y1)
-  **  ((&((t2_pre)  # "term" ->ₛ "content" .ₛ "Quant" .ₛ "var")) # Ptr  |-> y2)
-  **  ((&((t1_pre)  # "term" ->ₛ "type")) # Int  |-> (termtypeID (term1)))
-  **  ((&((t2_pre)  # "term" ->ₛ "type")) # Int  |-> (termtypeID (term2)))
-  **  ((&((t1_pre)  # "term" ->ₛ "content" .ₛ "Quant" .ₛ "type")) # Int  |-> (qtID (qt1)))
-  **  ((&((t2_pre)  # "term" ->ₛ "content" .ₛ "Quant" .ₛ "type")) # Int  |-> (qtID (qt2)))
-  **  ((&((t1_pre)  # "term" ->ₛ "content" .ₛ "Quant" .ₛ "body")) # Ptr  |-> z1)
-  **  ((&((t2_pre)  # "term" ->ₛ "content" .ₛ "Quant" .ₛ "body")) # Ptr  |-> z2)
-  **  (store_term z1 qterm1 )
-|--
-  [| (retval_3 = retval_2) |] 
-  &&  [| (retval_2 <> 0) |] 
-  &&  [| (y1 <> 0) |] 
-  &&  [| (y2 <> 0) |] 
-  &&  [| (retval <> 0) |] 
-  &&  [| (retval = (list_Z_cmp (qv1) (qv2))) |] 
-  &&  [| ((qtID (qt1)) = (qtID (qt2))) |] 
-  &&  [| (t1_pre <> 0) |] 
-  &&  [| (t2_pre <> 0) |] 
-  &&  [| (term1 = (TermQuant (qt1) (qv1) (qterm1))) |] 
-  &&  [| (term2 = (TermQuant (qt2) (qv2) (qterm2))) |] 
-  &&  [| ((termtypeID (term1)) = (termtypeID (term2))) |] 
-  &&  [| (t1_pre <> 0) |] 
-  &&  [| (t2_pre <> 0) |] 
-  &&  [| (t2_pre <> 0) |] 
-  &&  [| (t1_pre <> 0) |] 
-  &&  [| ((termtypeID (term1)) <> 0) |] 
-  &&  [| ((termtypeID (term1)) <> 1) |] 
-  &&  [| ((termtypeID (term1)) <> 2) |] 
-  &&  [| ((termtypeID (term1)) = 3) |]
-  &&  (store_term z1 qterm1 )
-  **  (store_term retval_3 (term_subst_v (qv1) (qv2) (qterm2)) )
-  **  (store_string y1 qv1 )
-  **  (store_string y2 qv2 )
-  **  (store_term z2 qterm2 )
-  **  ((&((t1_pre)  # "term" ->ₛ "content" .ₛ "Quant" .ₛ "var")) # Ptr  |-> y1)
-  **  ((&((t2_pre)  # "term" ->ₛ "content" .ₛ "Quant" .ₛ "var")) # Ptr  |-> y2)
-  **  ((&((t1_pre)  # "term" ->ₛ "type")) # Int  |-> (termtypeID (term1)))
-  **  ((&((t2_pre)  # "term" ->ₛ "type")) # Int  |-> (termtypeID (term2)))
-  **  ((&((t1_pre)  # "term" ->ₛ "content" .ₛ "Quant" .ₛ "type")) # Int  |-> (qtID (qt1)))
-  **  ((&((t2_pre)  # "term" ->ₛ "content" .ₛ "Quant" .ₛ "type")) # Int  |-> (qtID (qt2)))
   **  ((&((t1_pre)  # "term" ->ₛ "content" .ₛ "Quant" .ₛ "body")) # Ptr  |-> z1)
   **  ((&((t2_pre)  # "term" ->ₛ "content" .ₛ "Quant" .ₛ "body")) # Ptr  |-> z2)
 .
 
-Definition alpha_equiv_partial_solve_wit_15 := 
-forall (t2_pre: Z) (t1_pre: Z) (term2: term) (term1: term) (z2: Z) (z1: Z) (y2: Z) (y1: Z) (qt2: quant_type) (qv2: (@list Z)) (qterm2: term) (qt1: quant_type) (qv1: (@list Z)) (qterm1: term) (retval: Z) (retval_2: Z) (retval_3: Z) (retval_4: Z) ,
-  [| (retval_4 = (term_eqn (qterm1) ((term_subst_v (qv1) (qv2) (qterm2))))) |] 
-  &&  [| (retval_3 = retval_2) |] 
-  &&  [| (retval_2 <> 0) |] 
-  &&  [| (y1 <> 0) |] 
-  &&  [| (y2 <> 0) |] 
-  &&  [| (retval <> 0) |] 
-  &&  [| (retval = (list_Z_cmp (qv1) (qv2))) |] 
-  &&  [| ((qtID (qt1)) = (qtID (qt2))) |] 
-  &&  [| (t1_pre <> 0) |] 
-  &&  [| (t2_pre <> 0) |] 
-  &&  [| (term1 = (TermQuant (qt1) (qv1) (qterm1))) |] 
-  &&  [| (term2 = (TermQuant (qt2) (qv2) (qterm2))) |] 
-  &&  [| ((termtypeID (term1)) = (termtypeID (term2))) |] 
-  &&  [| (t1_pre <> 0) |] 
-  &&  [| (t2_pre <> 0) |] 
-  &&  [| (t2_pre <> 0) |] 
-  &&  [| (t1_pre <> 0) |] 
-  &&  [| ((termtypeID (term1)) <> 0) |] 
-  &&  [| ((termtypeID (term1)) <> 1) |] 
-  &&  [| ((termtypeID (term1)) <> 2) |] 
-  &&  [| ((termtypeID (term1)) = 3) |]
-  &&  (store_term z1 qterm1 )
-  **  (store_term retval_3 (term_subst_v (qv1) (qv2) (qterm2)) )
-  **  (store_string y1 qv1 )
-  **  (store_string y2 qv2 )
-  **  (store_term z2 qterm2 )
-  **  ((&((t1_pre)  # "term" ->ₛ "content" .ₛ "Quant" .ₛ "var")) # Ptr  |-> y1)
-  **  ((&((t2_pre)  # "term" ->ₛ "content" .ₛ "Quant" .ₛ "var")) # Ptr  |-> y2)
-  **  ((&((t1_pre)  # "term" ->ₛ "type")) # Int  |-> (termtypeID (term1)))
-  **  ((&((t2_pre)  # "term" ->ₛ "type")) # Int  |-> (termtypeID (term2)))
-  **  ((&((t1_pre)  # "term" ->ₛ "content" .ₛ "Quant" .ₛ "type")) # Int  |-> (qtID (qt1)))
-  **  ((&((t2_pre)  # "term" ->ₛ "content" .ₛ "Quant" .ₛ "type")) # Int  |-> (qtID (qt2)))
-  **  ((&((t1_pre)  # "term" ->ₛ "content" .ₛ "Quant" .ₛ "body")) # Ptr  |-> z1)
-  **  ((&((t2_pre)  # "term" ->ₛ "content" .ₛ "Quant" .ₛ "body")) # Ptr  |-> z2)
-|--
-  [| (retval_4 = (term_eqn (qterm1) ((term_subst_v (qv1) (qv2) (qterm2))))) |] 
-  &&  [| (retval_3 = retval_2) |] 
-  &&  [| (retval_2 <> 0) |] 
-  &&  [| (y1 <> 0) |] 
-  &&  [| (y2 <> 0) |] 
-  &&  [| (retval <> 0) |] 
-  &&  [| (retval = (list_Z_cmp (qv1) (qv2))) |] 
-  &&  [| ((qtID (qt1)) = (qtID (qt2))) |] 
-  &&  [| (t1_pre <> 0) |] 
-  &&  [| (t2_pre <> 0) |] 
-  &&  [| (term1 = (TermQuant (qt1) (qv1) (qterm1))) |] 
-  &&  [| (term2 = (TermQuant (qt2) (qv2) (qterm2))) |] 
-  &&  [| ((termtypeID (term1)) = (termtypeID (term2))) |] 
-  &&  [| (t1_pre <> 0) |] 
-  &&  [| (t2_pre <> 0) |] 
-  &&  [| (t2_pre <> 0) |] 
-  &&  [| (t1_pre <> 0) |] 
-  &&  [| ((termtypeID (term1)) <> 0) |] 
-  &&  [| ((termtypeID (term1)) <> 1) |] 
-  &&  [| ((termtypeID (term1)) <> 2) |] 
-  &&  [| ((termtypeID (term1)) = 3) |]
-  &&  (store_term retval_3 (term_subst_v (qv1) (qv2) (qterm2)) )
-  **  (store_term z1 qterm1 )
-  **  (store_string y1 qv1 )
-  **  (store_string y2 qv2 )
-  **  (store_term z2 qterm2 )
-  **  ((&((t1_pre)  # "term" ->ₛ "content" .ₛ "Quant" .ₛ "var")) # Ptr  |-> y1)
-  **  ((&((t2_pre)  # "term" ->ₛ "content" .ₛ "Quant" .ₛ "var")) # Ptr  |-> y2)
-  **  ((&((t1_pre)  # "term" ->ₛ "type")) # Int  |-> (termtypeID (term1)))
-  **  ((&((t2_pre)  # "term" ->ₛ "type")) # Int  |-> (termtypeID (term2)))
-  **  ((&((t1_pre)  # "term" ->ₛ "content" .ₛ "Quant" .ₛ "type")) # Int  |-> (qtID (qt1)))
-  **  ((&((t2_pre)  # "term" ->ₛ "content" .ₛ "Quant" .ₛ "type")) # Int  |-> (qtID (qt2)))
-  **  ((&((t1_pre)  # "term" ->ₛ "content" .ₛ "Quant" .ₛ "body")) # Ptr  |-> z1)
-  **  ((&((t2_pre)  # "term" ->ₛ "content" .ₛ "Quant" .ₛ "body")) # Ptr  |-> z2)
-.
+Definition alpha_equiv_partial_solve_wit_21 := alpha_equiv_partial_solve_wit_21_pure -> alpha_equiv_partial_solve_wit_21_aux.
 
 Definition alpha_equiv_which_implies_wit_1 := 
 forall (term2: term) (term1: term) (t1: Z) (t2: Z) ,
@@ -1783,18 +2432,50 @@ forall (term2: term) (term1: term) (t1: Z) (t2: Z) ,
 .
 
 Definition alpha_equiv_which_implies_wit_6 := 
-forall (qv2: (@list Z)) (qv1: (@list Z)) (t1: Z) (v: Z) (t2: Z) (v_2: Z) ,
-  ((&((t1)  # "term" ->ₛ "content" .ₛ "Quant" .ₛ "var")) # Ptr  |-> v)
-  **  (store_string v qv1 )
-  **  ((&((t2)  # "term" ->ₛ "content" .ₛ "Quant" .ₛ "var")) # Ptr  |-> v_2)
-  **  (store_string v_2 qv2 )
+forall (term2: term) (term1: term) (qterm2: term) (qv2: (@list Z)) (qt2: quant_type) (z2: Z) (y2: Z) (qterm1: term) (qv1: (@list Z)) (qt1: quant_type) (z1: Z) (y1: Z) (t1: Z) (t2: Z) ,
+  [| (t1 <> 0) |] 
+  &&  [| (t2 <> 0) |] 
+  &&  [| (term1 = (TermQuant (qt1) (qv1) (qterm1))) |] 
+  &&  [| (term2 = (TermQuant (qt2) (qv2) (qterm2))) |]
+  &&  ((&((t1)  # "term" ->ₛ "type")) # Int  |-> (termtypeID (term1)))
+  **  ((&((t2)  # "term" ->ₛ "type")) # Int  |-> (termtypeID (term2)))
+  **  ((&((t1)  # "term" ->ₛ "content" .ₛ "Quant" .ₛ "type")) # Int  |-> (qtID (qt1)))
+  **  ((&((t2)  # "term" ->ₛ "content" .ₛ "Quant" .ₛ "type")) # Int  |-> (qtID (qt2)))
+  **  ((&((t1)  # "term" ->ₛ "content" .ₛ "Quant" .ₛ "var")) # Ptr  |-> y1)
+  **  ((&((t2)  # "term" ->ₛ "content" .ₛ "Quant" .ₛ "var")) # Ptr  |-> y2)
+  **  ((&((t1)  # "term" ->ₛ "content" .ₛ "Quant" .ₛ "body")) # Ptr  |-> z1)
+  **  ((&((t2)  # "term" ->ₛ "content" .ₛ "Quant" .ₛ "body")) # Ptr  |-> z2)
+  **  (store_string y1 qv1 )
+  **  (store_term z1 qterm1 )
+  **  (store_string y2 qv2 )
+  **  (store_term z2 qterm2 )
 |--
-  [| (v <> 0) |] 
-  &&  [| (v_2 <> 0) |]
-  &&  ((&((t1)  # "term" ->ₛ "content" .ₛ "Quant" .ₛ "var")) # Ptr  |-> v)
-  **  ((&((t2)  # "term" ->ₛ "content" .ₛ "Quant" .ₛ "var")) # Ptr  |-> v_2)
-  **  (store_string v qv1 )
-  **  (store_string v_2 qv2 )
+  (store_term t1 term1 )
+  **  (store_term t2 term2 )
+.
+
+Definition alpha_equiv_which_implies_wit_7 := 
+forall (term2: term) (term1: term) (t1: Z) (t2: Z) ,
+  (store_term t1 term1 )
+  **  (store_term t2 term2 )
+|--
+  EX (z2: Z)  (z1: Z)  (y2: Z)  (y1: Z)  (qt2: quant_type)  (qv2: (@list Z))  (qterm2: term)  (qt1: quant_type)  (qv1: (@list Z))  (qterm1: term) ,
+  [| (t1 <> 0) |] 
+  &&  [| (t2 <> 0) |] 
+  &&  [| (term1 = (TermQuant (qt1) (qv1) (qterm1))) |] 
+  &&  [| (term2 = (TermQuant (qt2) (qv2) (qterm2))) |]
+  &&  ((&((t1)  # "term" ->ₛ "type")) # Int  |-> (termtypeID (term1)))
+  **  ((&((t2)  # "term" ->ₛ "type")) # Int  |-> (termtypeID (term2)))
+  **  ((&((t1)  # "term" ->ₛ "content" .ₛ "Quant" .ₛ "type")) # Int  |-> (qtID (qt1)))
+  **  ((&((t2)  # "term" ->ₛ "content" .ₛ "Quant" .ₛ "type")) # Int  |-> (qtID (qt2)))
+  **  ((&((t1)  # "term" ->ₛ "content" .ₛ "Quant" .ₛ "var")) # Ptr  |-> y1)
+  **  ((&((t2)  # "term" ->ₛ "content" .ₛ "Quant" .ₛ "var")) # Ptr  |-> y2)
+  **  ((&((t1)  # "term" ->ₛ "content" .ₛ "Quant" .ₛ "body")) # Ptr  |-> z1)
+  **  ((&((t2)  # "term" ->ₛ "content" .ₛ "Quant" .ₛ "body")) # Ptr  |-> z2)
+  **  (store_string y1 qv1 )
+  **  (store_term z1 qterm1 )
+  **  (store_string y2 qv2 )
+  **  (store_term z2 qterm2 )
 .
 
 Module Type VC_Correct.
@@ -1814,7 +2495,8 @@ Axiom proof_of_alpha_equiv_safety_wit_12 : alpha_equiv_safety_wit_12.
 Axiom proof_of_alpha_equiv_safety_wit_13 : alpha_equiv_safety_wit_13.
 Axiom proof_of_alpha_equiv_safety_wit_14 : alpha_equiv_safety_wit_14.
 Axiom proof_of_alpha_equiv_safety_wit_15 : alpha_equiv_safety_wit_15.
-Axiom proof_of_alpha_equiv_entail_wit_1 : alpha_equiv_entail_wit_1.
+Axiom proof_of_alpha_equiv_entail_wit_1_1 : alpha_equiv_entail_wit_1_1.
+Axiom proof_of_alpha_equiv_entail_wit_1_2 : alpha_equiv_entail_wit_1_2.
 Axiom proof_of_alpha_equiv_return_wit_1_1 : alpha_equiv_return_wit_1_1.
 Axiom proof_of_alpha_equiv_return_wit_1_2 : alpha_equiv_return_wit_1_2.
 Axiom proof_of_alpha_equiv_return_wit_2 : alpha_equiv_return_wit_2.
@@ -1826,10 +2508,9 @@ Axiom proof_of_alpha_equiv_return_wit_5_2 : alpha_equiv_return_wit_5_2.
 Axiom proof_of_alpha_equiv_return_wit_5_3 : alpha_equiv_return_wit_5_3.
 Axiom proof_of_alpha_equiv_return_wit_6 : alpha_equiv_return_wit_6.
 Axiom proof_of_alpha_equiv_return_wit_7 : alpha_equiv_return_wit_7.
-Axiom proof_of_alpha_equiv_return_wit_8 : alpha_equiv_return_wit_8.
-Axiom proof_of_alpha_equiv_return_wit_9_1 : alpha_equiv_return_wit_9_1.
-Axiom proof_of_alpha_equiv_return_wit_9_2 : alpha_equiv_return_wit_9_2.
-Axiom proof_of_alpha_equiv_return_wit_10 : alpha_equiv_return_wit_10.
+Axiom proof_of_alpha_equiv_return_wit_8_1 : alpha_equiv_return_wit_8_1.
+Axiom proof_of_alpha_equiv_return_wit_8_2 : alpha_equiv_return_wit_8_2.
+Axiom proof_of_alpha_equiv_return_wit_9 : alpha_equiv_return_wit_9.
 Axiom proof_of_alpha_equiv_partial_solve_wit_1 : alpha_equiv_partial_solve_wit_1.
 Axiom proof_of_alpha_equiv_partial_solve_wit_2_pure : alpha_equiv_partial_solve_wit_2_pure.
 Axiom proof_of_alpha_equiv_partial_solve_wit_2 : alpha_equiv_partial_solve_wit_2.
@@ -1844,17 +2525,27 @@ Axiom proof_of_alpha_equiv_partial_solve_wit_8_pure : alpha_equiv_partial_solve_
 Axiom proof_of_alpha_equiv_partial_solve_wit_8 : alpha_equiv_partial_solve_wit_8.
 Axiom proof_of_alpha_equiv_partial_solve_wit_9 : alpha_equiv_partial_solve_wit_9.
 Axiom proof_of_alpha_equiv_partial_solve_wit_10 : alpha_equiv_partial_solve_wit_10.
+Axiom proof_of_alpha_equiv_partial_solve_wit_11_pure : alpha_equiv_partial_solve_wit_11_pure.
 Axiom proof_of_alpha_equiv_partial_solve_wit_11 : alpha_equiv_partial_solve_wit_11.
 Axiom proof_of_alpha_equiv_partial_solve_wit_12 : alpha_equiv_partial_solve_wit_12.
-Axiom proof_of_alpha_equiv_partial_solve_wit_13_pure : alpha_equiv_partial_solve_wit_13_pure.
 Axiom proof_of_alpha_equiv_partial_solve_wit_13 : alpha_equiv_partial_solve_wit_13.
 Axiom proof_of_alpha_equiv_partial_solve_wit_14 : alpha_equiv_partial_solve_wit_14.
+Axiom proof_of_alpha_equiv_partial_solve_wit_15_pure : alpha_equiv_partial_solve_wit_15_pure.
 Axiom proof_of_alpha_equiv_partial_solve_wit_15 : alpha_equiv_partial_solve_wit_15.
+Axiom proof_of_alpha_equiv_partial_solve_wit_16 : alpha_equiv_partial_solve_wit_16.
+Axiom proof_of_alpha_equiv_partial_solve_wit_17_pure : alpha_equiv_partial_solve_wit_17_pure.
+Axiom proof_of_alpha_equiv_partial_solve_wit_17 : alpha_equiv_partial_solve_wit_17.
+Axiom proof_of_alpha_equiv_partial_solve_wit_18 : alpha_equiv_partial_solve_wit_18.
+Axiom proof_of_alpha_equiv_partial_solve_wit_19 : alpha_equiv_partial_solve_wit_19.
+Axiom proof_of_alpha_equiv_partial_solve_wit_20 : alpha_equiv_partial_solve_wit_20.
+Axiom proof_of_alpha_equiv_partial_solve_wit_21_pure : alpha_equiv_partial_solve_wit_21_pure.
+Axiom proof_of_alpha_equiv_partial_solve_wit_21 : alpha_equiv_partial_solve_wit_21.
 Axiom proof_of_alpha_equiv_which_implies_wit_1 : alpha_equiv_which_implies_wit_1.
 Axiom proof_of_alpha_equiv_which_implies_wit_2 : alpha_equiv_which_implies_wit_2.
 Axiom proof_of_alpha_equiv_which_implies_wit_3 : alpha_equiv_which_implies_wit_3.
 Axiom proof_of_alpha_equiv_which_implies_wit_4 : alpha_equiv_which_implies_wit_4.
 Axiom proof_of_alpha_equiv_which_implies_wit_5 : alpha_equiv_which_implies_wit_5.
 Axiom proof_of_alpha_equiv_which_implies_wit_6 : alpha_equiv_which_implies_wit_6.
+Axiom proof_of_alpha_equiv_which_implies_wit_7 : alpha_equiv_which_implies_wit_7.
 
 End VC_Correct.
