qcp/ast/lib/ast_lib.v
@@ -506,7 +506,7 @@ Proof.
   intros. apply common_free_var_fresh.
 Qed.
 
-Fixpoint term_size (t: term) : Z :=
+(* Fixpoint term_size (t: term) : Z :=
   match t with
   | TermVar _ => 1
   | TermConst _ _ => 1
@@ -534,30 +534,7 @@ Proof.
   + fold term_subst_v in *.
     destruct (list_Z_eqb qvar new) eqn:Heq; [reflexivity | ].
     unfold term_size; fold term_size; lia.
-Qed.
-
-Inductive term_alpha_eq : term -> term -> Prop :=
-  | AlphaVar : forall v1 v2,
-      v1 = v2 ->
-      term_alpha_eq (TermVar v1) (TermVar v2)
-  | AlphaConst : forall ctype1 content1 ctype2 content2,
-      ctID ctype1 = ctID ctype2 ->
-      (ctID ctype1 <> 0 \/ content1 = content2) ->
-      term_alpha_eq (TermConst ctype1 content1) (TermConst ctype2 content2)
-  | AlphaApply : forall lt1 rt1 lt2 rt2,
-      term_alpha_eq lt1 lt2 -> term_alpha_eq rt1 rt2 ->
-      term_alpha_eq (TermApply lt1 rt1) (TermApply lt2 rt2)
-  | AlphaQuant : forall qtype1 qvar1 body1 qtype2 qvar2 body2,
-      qtID qtype1 = qtID qtype2 ->
-      (list_Z_eqb qvar1 qvar2 = true) /\ (term_alpha_eq body1 body2) \/
-      (exists fresh,
-        term_not_contain_var (TermQuant qtype1 qvar1 body1) fresh /\
-        term_not_contain_var (TermQuant qtype2 qvar2 body2) fresh /\
-        term_alpha_eq 
-          (term_subst_v fresh qvar1 body1) 
-          (term_subst_v fresh qvar2 body2)) ->
-      term_alpha_eq (TermQuant qtype1 qvar1 body1) (TermQuant qtype2 qvar2 body2).
-
+Qed. *)
 
 (* Program Fixpoint term_alpha_eq (t1 t2: term) 
   {measure (Z.to_nat (term_size t1))} : Prop :=
@@ -579,9 +556,6 @@ Inductive term_alpha_eq : term -> term -> Prop :=
   | _, _ => False
   end.
 Admit Obligations. *)
-
-Definition term_eqn (t1 t2: term): Prop :=
-  term_alpha_eq t1 t2.
 
 Fixpoint sub_thm (thm: term) (l: var_sub_list): term :=
   match l with 
@@ -670,6 +644,153 @@ Proof.
   reflexivity.
 Qed.
 
+Inductive term_alpha_eq : term -> term -> Prop :=
+  | AlphaVar : forall v1 v2,
+      v1 = v2 ->
+      term_alpha_eq (TermVar v1) (TermVar v2)
+  | AlphaConst : forall ctype1 content1 ctype2 content2,
+      ctID ctype1 = ctID ctype2 ->
+      (ctID ctype1 <> 0 \/ content1 = content2) ->
+      term_alpha_eq (TermConst ctype1 content1) (TermConst ctype2 content2)
+  | AlphaApply : forall lt1 rt1 lt2 rt2,
+      term_alpha_eq lt1 lt2 -> term_alpha_eq rt1 rt2 ->
+      term_alpha_eq (TermApply lt1 rt1) (TermApply lt2 rt2)
+  | AlphaQuant : forall qtype1 qvar1 body1 qtype2 qvar2 body2,
+      qtID qtype1 = qtID qtype2 ->
+      (list_Z_eqb qvar1 qvar2 = true) /\ (term_alpha_eq body1 body2) \/
+      (term_alpha_eq body1 (term_subst_v qvar1 qvar2 body2)) /\
+      (term_alpha_eq (term_subst_v qvar2 qvar1 body1) body2) ->
+      term_alpha_eq (TermQuant qtype1 qvar1 body1) (TermQuant qtype2 qvar2 body2).
+
+Fixpoint term_eq (t1 t2: term) : bool :=
+  match t1, t2 with
+  | TermVar v1, TermVar v2 => 
+      list_Z_eqb v1 v2
+  | TermConst ctype1 content1, TermConst ctype2 content2 =>
+      (Z.eqb (ctID ctype1) (ctID ctype2)) && 
+      ((negb (Z.eqb (ctID ctype1) 0)) || (Z.eqb content1 content2)) 
+  | TermApply lt1 rt1, TermApply lt2 rt2 =>
+      term_eq lt1 lt2 && term_eq rt1 rt2
+  | TermQuant qtype1 qvar1 body1, TermQuant qtype2 qvar2 body2 =>
+      (Z.eqb (qtID qtype1) (qtID qtype2)) && (list_Z_eqb qvar1 qvar2) &&
+      term_eq body1 body2
+  | _, _ => false
+  end.
+
+Lemma term_eq_refl: forall t,
+  term_eq t t = true.
+Proof.
+  induction t.
+  + unfold term_eq; apply list_Z_eq2eqb; reflexivity.
+  + unfold term_eq; rewrite andb_true_iff.
+    split.
+    - rewrite Z.eqb_eq; reflexivity.
+    - rewrite orb_true_iff.
+      right.
+      rewrite Z.eqb_eq; reflexivity.
+  + unfold term_eq; fold term_eq.
+    rewrite andb_true_iff.
+    auto.
+  + unfold term_eq; fold term_eq.
+    rewrite andb_true_iff.
+    rewrite andb_true_iff.
+    split. split.
+    - rewrite Z.eqb_eq; reflexivity.
+    - apply list_Z_eq2eqb; reflexivity.
+    - auto.
+Qed.  
+
+Lemma term_eq_symm: forall t1 t2,
+  term_eq t1 t2 = true -> term_eq t2 t1 = true.
+Proof.
+  induction t1,t2; try discriminate.
+  + unfold term_eq.
+    apply list_Z_eqb_symm.
+  + unfold term_eq.
+    rewrite andb_true_iff.
+    rewrite orb_true_iff.
+    intros.
+    rewrite andb_true_iff.
+    rewrite orb_true_iff.
+    destruct H as [Ha [Hb|Hc]].
+    - split.
+      * rewrite Z.eqb_eq in *; auto.
+      * rewrite negb_true_iff in *.
+        rewrite Z.eqb_eq in Ha.
+        rewrite <- Ha.
+        left; auto.
+    - split.
+      * rewrite Z.eqb_eq in *; auto.
+      * rewrite Z.eqb_eq in *.
+        right; auto.
+  + unfold term_eq in * ; fold term_eq in *.
+    rewrite andb_true_iff.
+    rewrite andb_true_iff.
+    intros.
+    destruct H as [Ha Hb].
+    pose proof IHt1_1 t2_1 Ha.
+    pose proof IHt1_2 t2_2 Hb.
+    auto.
+  + unfold term_eq in * ; fold term_eq in *.
+    repeat rewrite andb_true_iff in *.
+    intros.
+    destruct H as [[Ha Hb] Hc].
+    rewrite Z.eqb_eq in *.
+    split. split.
+    - auto.
+    - apply list_Z_eqb_symm; auto.
+    - apply (IHt1 t2 Hc).
+Qed.
+
+Lemma term_eq_trans: forall t1 t2 t3,
+  term_eq t1 t2 = true ->
+  term_eq t2 t3 = true ->
+  term_eq t1 t3 = true.
+Proof.
+  intros t1 t2.
+  revert t1.
+  induction t2.
+  + destruct t1, t3; try discriminate.
+    unfold term_eq.
+    apply list_Z_eqb_trans.
+  + destruct t1, t3; try discriminate.
+    unfold term_eq.
+    repeat rewrite andb_true_iff, orb_true_iff.
+    rewrite Z.eqb_eq.
+    intros.
+    destruct H as [Ha [Hb|Hc]].
+    rewrite Ha in *.
+    destruct H0 as [H1a [H1b|H1c]].
+    - split; auto.
+    - split; auto.
+    - destruct H0 as [H1a [H1b|H1c]].
+      * repeat rewrite negb_true_iff, Z.eqb_eq, Z.eqb_neq in *.
+        split. rewrite Ha, H1a; reflexivity.
+        left; rewrite Ha; auto.
+      * repeat rewrite negb_true_iff, Z.eqb_eq, Z.eqb_neq in *.
+        split. rewrite Ha, H1a; reflexivity.
+        right. rewrite Z.eqb_eq, Hc, H1c; reflexivity.
+  + destruct t1, t3; try discriminate.
+    unfold term_eq; fold term_eq.
+    intros.
+    repeat rewrite andb_true_iff in *.
+    destruct H, H0.
+    split.
+    apply (IHt2_1 t1_1 t3_1 H H0).
+    apply (IHt2_2 t1_2 t3_2 H1 H2).
+  + destruct t1, t3; try discriminate.
+    unfold term_eq; fold term_eq.
+    intros.
+    repeat rewrite andb_true_iff in *.
+    destruct H, H0.
+    destruct H, H0.
+    split. split.
+    - rewrite Z.eqb_eq in *.
+      rewrite H, H0; reflexivity.
+    - apply (list_Z_eqb_trans qvar0 qvar qvar1); try auto.
+    - apply (IHt2 t1 t3 H1 H2). 
+Qed.
+
 Lemma term_alpha_eq_refl : forall (t : term),
   term_alpha_eq t t.
 Proof.
@@ -710,10 +831,9 @@ Proof.
       * apply H10, H8.
     - right.
       destruct H7 as [x Hx].
-      exists x.
-      destruct Hx as [Hxa [Hxb Hxc]].
-      split; auto. 
-      split; auto. 
+      split.
+      * admit.
+      * apply (IHt1 (term_subst_v qvar qvar0 t2) x).
 Admitted.
 
 Lemma term_alpha_eq_trans : forall (t1 t2 t3 : term),
